@prefix : <http://www.fortiss.org/diprolea/ontosustain/rso#> .
@prefix dc: <http://purl.org/dc/elements/1.1/> .
@prefix dct: <http://purl.org/dc/terms/> .
@prefix gri: <http://www.fortiss.org/diprolea/ontosustain/rsr/gri#> .
@prefix owl: <http://www.w3.org/2002/07/owl#> .
@prefix rdf: <http://www.w3.org/1999/02/22-rdf-syntax-ns#> .
@prefix rso: <http://www.fortiss.org/diprolea/ontosustain/rso#> .
@prefix rsr: <http://www.fortiss.org/diprolea/ontosustain/rsr#> .
@prefix xml: <http://www.w3.org/XML/1998/namespace> .
@prefix xsd: <http://www.w3.org/2001/XMLSchema#> .
@prefix core: <http://www.fortiss.org/diprolea/ontosustain/rsr/core#> .
@prefix dcam: <http://purl.org/dc/dcam/> .
@prefix esrs: <http://www.fortiss.org/diprolea/ontosustain/rsr/esrs#> .
@prefix qudt: <http://qudt.org/schema/qudt/> .
@prefix rdfs: <http://www.w3.org/2000/01/rdf-schema#> .
@prefix skos: <http://www.w3.org/2004/02/skos/core#> .
@prefix unit: <http://qudt.org/vocab/unit/> .
@prefix vann: <http://purl.org/vocab/vann/> .
@prefix report: <http://www.fortiss.org/diprolea/ontosustain/rsr/report#> .
@prefix schema: <https://schema.org/> .
@prefix quantitykind: <http://qudt.org/vocab/quantitykind/> .
@base <http://www.fortiss.org/diprolea/ontosustain/rso#> .

<http://www.fortiss.org/diprolea/ontosustain/rso> rdf:type owl:Ontology ;
                                                   dc:publisher "fortissGmbH, Platfrom Engineering Group"@en ;
                                                   dc:title "An Ontology towards Digital Sustainability Reporting"@en ;
                                                   dct:abstract "Sustainability reporting by Small and Medium Enterprises (SMEs) is gaining importance. SMEs form the backbone of European industries, and their customers rely on them to ensure regulatory compliance. In preparing sustainability reports, a combination of standards is commonly used, which encompasses overlapping yet distinct requirements on sustainability indicators. Different standards categorize shared indicators under varying topics, while they also mandate unique indicators to assess identical sustainability phenomena. This poses challenges for SMEs in reporting against multiple standards. Considerable human efforts are demanded to determine the interconnected requirements across different standards. Additionally, reporting on overlapping indicators for new standards results in significant redundant work. Mapping of indicators between different standards allows the semantic interoperability of standards by indicating matching and distinct requirements, aiding in addressing these challenges. The purpose of RSO is to facilitate the interoperability of sustainability standards by indicating the matching and distinct indicators. Indicator mapping will provide further information such as: which report data can be reused for another standard, what distinct requirements exist for the overlapping indicators in two standards, and which distinct indicators are required for the same topic/subtopic by different standards."@en ;
                                                   dct:contributor "https://orcid.org/0000-0002-5881-3608" ,
                                                                   "https://orcid.org/0009-0006-1763-7544" ;
                                                   dct:created "2023-12-01" ;
                                                   dct:creator "https://orcid.org/0009-0003-0305-9622" ;
                                                   dct:description "RSO is designed  for mapping quantitative environmental indicators from the two significant sustainability reporting standards, GRI and ESRS. It formally represents (1) the classification and provenance information of indicators in the GRI and ESRS standards; (2) the requirements for indicators. RSO is envisioned to be integrated into the SME digital infrastructure. Accompanied by suitable digital infrastructure, the reporting system leveraging RSO as a knowledge base will empower the daily tasks of sustainability managers."@en ,
                                                                   "The ontology defines the representation of environmental indicators in sustainability reporting standards GRI and ESRS."@en ;
                                                   dct:license <https://creativecommons.org/licenses/by/4.0/> ;
                                                   vann:preferredNamespacePrefix "rso" ;
                                                   vann:preferredNamespaceUri "http://www.fortiss.org/diprolea/ontosustain/rso#" ;
                                                   rdfs:comment "RSO is designed for mapping quantitative environmental indicators from the two significant sustainability reporting standards, GRI and ESRS. It formally represents (1) the classification and provenance information of indicators in the GRI and ESRS standards; (2) the requirements for indicators. RSO is envisioned to be integrated into the SME digital infrastructure. Accompanied by suitable digital infrastructure, the reporting system leveraging RSO as a knowledge base will empower the daily tasks of sustainability managers."@en ;
                                                   rdfs:label "The Sustainability Reporting Standard Ontology"@en ;
                                                   owl:versionIRI "http://www.fortiss.org/diprolea/ontosustain/rso/0.1.0" ;
                                                   owl:versionInfo "0.1.0" ;
                                                   schema:url "http://www.fortiss.org/diprolea/ontosustain/rso" .

#################################################################
#    Annotation properties
#################################################################

###  http://purl.org/dc/elements/1.1/identifier
dc:identifier rdf:type owl:AnnotationProperty ;
              rdfs:range xsd:string .


###  http://purl.org/dc/elements/1.1/publisher
dc:publisher rdf:type owl:AnnotationProperty .


###  http://purl.org/dc/elements/1.1/title
dc:title rdf:type owl:AnnotationProperty .


###  http://purl.org/dc/terms/abstract
dct:abstract rdf:type owl:AnnotationProperty .


###  http://purl.org/dc/terms/contributor
dct:contributor rdf:type owl:AnnotationProperty .


###  http://purl.org/dc/terms/created
dct:created rdf:type owl:AnnotationProperty .


###  http://purl.org/dc/terms/creator
dct:creator rdf:type owl:AnnotationProperty .


###  http://purl.org/dc/terms/description
dct:description rdf:type owl:AnnotationProperty .


###  http://purl.org/dc/terms/license
dct:license rdf:type owl:AnnotationProperty .


###  http://purl.org/dc/terms/title
dct:title rdf:type owl:AnnotationProperty .


###  http://purl.org/vocab/vann/preferredNamespacePrefix
vann:preferredNamespacePrefix rdf:type owl:AnnotationProperty .


###  http://purl.org/vocab/vann/preferredNamespaceUri
vann:preferredNamespaceUri rdf:type owl:AnnotationProperty .


###  http://www.fortiss.org/diprolea/ontosustain/rso#hasOfficialCode
rso:hasOfficialCode rdf:type owl:AnnotationProperty .


###  http://www.fortiss.org/diprolea/ontosustain/rso#hasSelfDefinedCode
rso:hasSelfDefinedCode rdf:type owl:AnnotationProperty .


###  http://www.w3.org/2002/07/owl#versionIRI
owl:versionIRI rdf:type owl:AnnotationProperty .


###  http://www.w3.org/2004/02/skos/core#definition
skos:definition rdf:type owl:AnnotationProperty .


###  http://www.w3.org/2004/02/skos/core#prefLabel
skos:prefLabel rdf:type owl:AnnotationProperty .


###  https://schema.org/url
schema:url rdf:type owl:AnnotationProperty .


#################################################################
#    Object Properties
#################################################################

###  http://qudt.org/schema/qudt/hasQuantityKind
qudt:hasQuantityKind rdf:type owl:ObjectProperty ;
                     rdfs:domain [ rdf:type owl:Class ;
                                   owl:unionOf ( qudt:Unit
                                                 rso:Indicator
                                               )
                                 ] ;
                     rdfs:range qudt:QuantityKind ;
                     rdfs:comment "This property relates the indicator with the required quantity kind derived from the sustainability standards."@en ;
                     rdfs:label "has Quantity Kind"@en ;
                     skos:prefLabel "has Quantity Kind"@en .


###  http://www.fortiss.org/diprolea/ontosustain/rso#hasApplicability
rso:hasApplicability rdf:type owl:ObjectProperty ;
                     rdfs:domain rso:Indicator ;
                     rdfs:range rso:Applicability ;
                     rdfs:comment "This property relates the indicator with the indicator applicability derived from the sustainability standards (either mandatory, optional, or enumerated)."@en ;
                     rdfs:label "has applicability"@en ;
                     skos:prefLabel "has applicability"@en .


###  http://www.fortiss.org/diprolea/ontosustain/rso#hasBreakDownValue
rso:hasBreakDownValue rdf:type owl:ObjectProperty ;
                      rdfs:domain rso:ReportValue ;
                      rdfs:range rso:BreakDownValue ;
                      rdfs:comment "This property links a report value with several break down values."@en ;
                      rdfs:label "has break down value"@en ;
                      skos:prefLabel "has break down value"@en .


###  http://www.fortiss.org/diprolea/ontosustain/rso#hasCalculationVariable
rso:hasCalculationVariable rdf:type owl:ObjectProperty ;
                           rdfs:domain rso:AbsoluteIndicator ;
                           rdfs:range rso:Variable ;
                           rdfs:comment "This property relates the indicator to the required variables for calculating its value, as defined by mathematical functions in the sustainability standards."@en ;
                           rdfs:label "has Calculation Variable"@en ;
                           skos:prefLabel "has Calculation Variable"@en .


###  http://www.fortiss.org/diprolea/ontosustain/rso#hasDenominatorQuantityKind
rso:hasDenominatorQuantityKind rdf:type owl:ObjectProperty ;
                               rdfs:subPropertyOf qudt:hasQuantityKind ;
                               rdfs:domain rso:IntensityIndicator ;
                               rdfs:range qudt:QuantityKind ;
                               rdfs:comment "This property relates the intensity indicator with the required quantity kind of the denominator derived from the sustainability standards."@en ;
                               rdfs:label "has Denominator Quantity Kind"@en ;
                               skos:prefLabel "has Denominator Quantity Kind"@en .


###  http://www.fortiss.org/diprolea/ontosustain/rso#hasDenominatorVariable
rso:hasDenominatorVariable rdf:type owl:ObjectProperty ;
                           rdfs:subPropertyOf rso:hasMeasurementVariable ;
                           rdfs:domain rso:WeightedIndicator ;
                           rdfs:range rso:Variable ;
                           rdfs:comment "This property relates the weighted indicator with the measurement variable (object) of the denominator derived from the sustainability standards."@en ;
                           rdfs:label "has Denominator Variable"@en ;
                           skos:prefLabel "has Denominator Variable"@en .


###  http://www.fortiss.org/diprolea/ontosustain/rso#hasMeasurementVariable
rso:hasMeasurementVariable rdf:type owl:ObjectProperty ;
                           rdfs:domain rso:Indicator ;
                           rdfs:range rso:Variable ;
                           rdfs:comment "This property relates the indicator with the measurement variable (object) derived from the sustainability standards."@en ;
                           rdfs:label "has Measurement Variable"@en ;
                           skos:prefLabel "has Measurement Variable"@en .


###  http://www.fortiss.org/diprolea/ontosustain/rso#hasNegativeVariable
rso:hasNegativeVariable rdf:type owl:ObjectProperty ;
                        rdfs:subPropertyOf rso:hasCalculationVariable ;
                        rdfs:domain rso:AbsoluteIndicator ;
                        rdfs:range rso:Variable ;
                        rdfs:comment "This property relates the indicator to the required variables for calculating its value, if the defined mathematical symbol is minus."@en ;
                        rdfs:label "has Negative Variable"@en ;
                        skos:prefLabel "has Negative Variable"@en .


###  http://www.fortiss.org/diprolea/ontosustain/rso#hasNumeratorQuantityKind
rso:hasNumeratorQuantityKind rdf:type owl:ObjectProperty ;
                             rdfs:subPropertyOf qudt:hasQuantityKind ;
                             rdfs:domain rso:IntensityIndicator ;
                             rdfs:range qudt:QuantityKind ;
                             rdfs:comment "This property relates the intensity indicator with the required quantity kind of the numerator derived from the sustainability standards."@en ;
                             rdfs:label "has Numerator Quantity Kind"@en ;
                             skos:prefLabel "has Numerator Quantity Kind"@en .


###  http://www.fortiss.org/diprolea/ontosustain/rso#hasNumeratorVariable
rso:hasNumeratorVariable rdf:type owl:ObjectProperty ;
                         rdfs:subPropertyOf rso:hasMeasurementVariable ;
                         rdfs:domain rso:WeightedIndicator ;
                         rdfs:range rso:Variable ;
                         rdfs:comment "This property relates the weighted indicator with the measurement variable (object) of the numerator derived from the sustainability standards."@en ;
                         rdfs:label "has Numerator Variable"@en ;
                         skos:prefLabel "has Numerator Variable"@en .


###  http://www.fortiss.org/diprolea/ontosustain/rso#hasPositiveVariable
rso:hasPositiveVariable rdf:type owl:ObjectProperty ;
                        rdfs:subPropertyOf rso:hasCalculationVariable ;
                        rdfs:domain rso:AbsoluteIndicator ;
                        rdfs:range rso:Variable ;
                        rdfs:comment "This property relates the indicator to the required variables for calculating its value, if the defined mathematical symbol is plus."@en ;
                        rdfs:label "has Positive Variable"@en ;
                        skos:prefLabel "has Positive Variable"@en .


###  http://www.fortiss.org/diprolea/ontosustain/rso#hasReportValue
rso:hasReportValue rdf:type owl:ObjectProperty ;
                   rdfs:domain rso:Report ;
                   rdfs:range rso:ReportValue ;
                   rdfs:comment "This property links the sustainability report with the report value."@en ;
                   rdfs:label "has report value"@en ;
                   skos:prefLabel "has report value"@en .


###  http://www.fortiss.org/diprolea/ontosustain/rso#hasSiblingIndicator
rso:hasSiblingIndicator rdf:type owl:ObjectProperty ;
                        rdfs:subPropertyOf owl:topObjectProperty ;
                        rdf:type owl:SymmetricProperty ;
                        rdfs:domain rso:Indicator ;
                        rdfs:range rso:Indicator ;
                        rdfs:comment "This property relates the indicators defined by the same standard setter with the same measurement variable but different quantity kind. This property is defined as a symmetric property."@en ;
                        rdfs:label "has Sibling Indicator"@en ;
                        skos:prefLabel "has Sibling Indicator"@en .


###  http://www.fortiss.org/diprolea/ontosustain/rso#inDisclosure
rso:inDisclosure rdf:type owl:ObjectProperty ;
                 rdfs:domain rso:GRIIndicator ;
                 rdfs:range rso:GRIDisclosure ;
                 rdfs:comment "This property relates a GRI indicator with the corresponding disclosure that defines this indicator in the GRI standards."@en ;
                 rdfs:label "in GRI Disclosure"@en ;
                 skos:prefLabel "in GRI Disclosure"@en .


###  http://www.fortiss.org/diprolea/ontosustain/rso#inDisclosureRequirement
rso:inDisclosureRequirement rdf:type owl:ObjectProperty ;
                            rdfs:domain rso:ESRSIndicator ;
                            rdfs:range rso:ESRSDisclosureRequirement ;
                            rdfs:comment """User
This property relates an ESRS indicator with the corresponding ESRS Disclosure Requirement from where this indicator was derived."""@en ;
                            rdfs:label "in ESRS disclosure requirement"@en ;
                            skos:prefLabel "in ESRS disclosure requirement"@en .


###  http://www.fortiss.org/diprolea/ontosustain/rso#inStandard
rso:inStandard rdf:type owl:ObjectProperty ;
               rdfs:domain [ rdf:type owl:Class ;
                             owl:unionOf ( rso:Disclosure
                                           rso:Indicator
                                           rso:Topic
                                         )
                           ] ;
               rdfs:range rso:Standard ;
               rdfs:comment "This property relates an indicator, a topic,  or a disclosure / disclosure requirement with the specific piece of either GRI standard or ESRS standard that defines this indicator or this disclosure."@en ;
               rdfs:label "in sustainability standard"@en ;
               skos:prefLabel "in sustainability standard"@en .


###  http://www.fortiss.org/diprolea/ontosustain/rso#isDefinedBy
rso:isDefinedBy rdf:type owl:ObjectProperty ;
                rdfs:domain [ rdf:type owl:Class ;
                              owl:unionOf ( rso:Disclosure
                                            rso:Indicator
                                            rso:Topic
                                          )
                            ] ;
                rdfs:range rso:StandardSet ;
                rdfs:comment "This property relates an indicator or a piece of standard with the specific standard set (either GRI or ESRS) that defines it."@en ;
                rdfs:label "is Defined By"@en ;
                skos:definition "is Defined By"@en .


###  http://www.fortiss.org/diprolea/ontosustain/rso#measuresCoreTopic
rso:measuresCoreTopic rdf:type owl:ObjectProperty ;
                      rdfs:subPropertyOf rso:measuresTopic ;
                      rdfs:domain rso:Indicator ;
                      rdfs:range rso:CoreTopic ;
                      rdfs:comment "This property relates the indicator with certain Core Topic that the indicator measures."@en ;
                      rdfs:label "measures Core topic"@en ;
                      skos:prefLabel "measures Core topic"@en .


###  http://www.fortiss.org/diprolea/ontosustain/rso#measuresDimension
rso:measuresDimension rdf:type owl:ObjectProperty ;
                      rdfs:domain rso:Indicator ;
                      rdfs:range rso:ESGDimension ;
                      rdfs:comment "This property relates the indicator with the ESG dimension (either Environmental, Social, or corporate Goverment) that the indicator measures."@en ;
                      rdfs:label "measures ESG dimension"@en ;
                      skos:prefLabel "measures ESG dimension"@en .


###  http://www.fortiss.org/diprolea/ontosustain/rso#measuresESRSTopic
rso:measuresESRSTopic rdf:type owl:ObjectProperty ;
                      rdfs:subPropertyOf rso:measuresTopic ;
                      rdfs:domain rso:ESRSIndicator ;
                      rdfs:range rso:ESRSTopic ;
                      rdfs:comment "This property relates the indicator with certain ESRS Topic that the indicator measures."@en ;
                      rdfs:label "measures ESRS Topic"@en ;
                      skos:prefLabel "measures ESRS Topic"@en .


###  http://www.fortiss.org/diprolea/ontosustain/rso#measuresGRITopic
rso:measuresGRITopic rdf:type owl:ObjectProperty ;
                     rdfs:subPropertyOf rso:measuresTopic ;
                     rdfs:domain rso:GRIIndicator ;
                     rdfs:range rso:GRITopic ;
                     rdfs:comment "This property relates the indicator with certain GRI Topic that the indicator measures."@en ;
                     rdfs:label "measures GRI Topic"@en ;
                     skos:prefLabel "measures GRI Topic"@en .


###  http://www.fortiss.org/diprolea/ontosustain/rso#measuresTopic
rso:measuresTopic rdf:type owl:ObjectProperty ;
                  rdfs:domain rso:Indicator ;
                  rdfs:range rso:Topic ;
                  rdfs:comment "This property relates the indicator with specific sustainability topic that the indicator measures."@en ;
                  rdfs:label "measures sustainability topic"@en ;
                  skos:prefLabel "measures sustainability topic"@en .


###  http://www.fortiss.org/diprolea/ontosustain/rso#publish
rso:publish rdf:type owl:ObjectProperty ;
            rdfs:domain <http://www.w3.org/ns/org#Organization> ;
            rdfs:range rso:Report ;
            rdfs:comment "This property links an organization to the sustainability reports published by it."@en ;
            rdfs:label "publish"@en ;
            skos:prefLabel "publish"@en .


###  http://www.fortiss.org/diprolea/ontosustain/rso#reportsOnIndicator
rso:reportsOnIndicator rdf:type owl:ObjectProperty ;
                       rdfs:domain rso:ReportValue ;
                       rdfs:range rso:Indicator ;
                       rdfs:comment "This property associates a reported value with the particular indicator derived from the standards, which the value represents."@en ;
                       rdfs:label "reports on indicator"@en ;
                       skos:prefLabel "reports on indicator"@en .


###  https://qudt.org/schema/qudt/hasUnit
<https://qudt.org/schema/qudt/hasUnit> rdf:type owl:ObjectProperty ;
                                       rdfs:domain [ rdf:type owl:Class ;
                                                     owl:unionOf ( rso:Indicator
                                                                   rso:Value
                                                                 )
                                                   ] ;
                                       rdfs:range qudt:Unit ;
                                       rdfs:comment "This property relates the indicator with the required unit derived from the sustainability standards."@en ;
                                       rdfs:label "has Unit"@en ;
                                       skos:prefLabel "has Unit"@en .


#################################################################
#    Data properties
#################################################################

###  http://www.fortiss.org/diprolea/ontosustain/rso#hasNumericalValue
rso:hasNumericalValue rdf:type owl:DatatypeProperty ;
                      rdfs:subPropertyOf owl:topDataProperty ;
                      rdfs:domain rso:Value ;
                      rdfs:range xsd:decimal ;
                      rdfs:comment "This property relates the indicator value with its specific numerical value."@en ;
                      rdfs:label "has Numerical Value"@en ;
                      skos:prefLabel "has Numerical Value"@en .


###  http://www.fortiss.org/diprolea/ontosustain/rso#hasYear
rso:hasYear rdf:type owl:DatatypeProperty ;
            rdfs:subPropertyOf owl:topDataProperty ;
            rdfs:domain rso:Report ;
            rdfs:range xsd:string ;
            rdfs:comment "This property links the sustainability report to its publication year."@en ;
            rdfs:label "has Year"@en ;
            skos:prefLabel "has Year"@en .


#################################################################
#    Classes
#################################################################

###  http://qudt.org/schema/qudt/QuantityKind
qudt:QuantityKind rdf:type owl:Class .


###  http://qudt.org/schema/qudt/Unit
qudt:Unit rdf:type owl:Class .


###  http://www.fortiss.org/diprolea/ontosustain/rso#AbsoluteIndicator
rso:AbsoluteIndicator rdf:type owl:Class ;
                      rdfs:subClassOf rso:Indicator ;
                      owl:disjointWith rso:WeightedIndicator ;
                      rdfs:comment "Absolute indicator represents the total quantity of a phenomenon."@en ;
                      rdfs:label "Absolute Indicator"@en ;
                      skos:prefLabel "Absolute Indicator"@en .


###  http://www.fortiss.org/diprolea/ontosustain/rso#Applicability
rso:Applicability rdf:type owl:Class ;
                  owl:equivalentClass [ rdf:type owl:Class ;
                                        owl:oneOf ( rso:enumerated
                                                    rso:mandatory
                                                    rso:optional
                                                  )
                                      ] ;
                  rdfs:comment "Indicates whether an indicator is required mandatorily or optionally by the corresponding standard."@en ;
                  rdfs:label "Indicator Requirement Applicability"@en ;
                  skos:prefLabel "Indicator Requirement Applicability"@en .


###  http://www.fortiss.org/diprolea/ontosustain/rso#BreakDownValue
rso:BreakDownValue rdf:type owl:Class ;
                   rdfs:subClassOf rso:Value ;
                   rdfs:comment """Breakdown values are crafted to meet the standards' requirements, allowing organizations to dissect a total report value based on specific criteria. 
These breakdown values are linked to specific report values."""@en ;
                   rdfs:label "Break Down Value"@en ;
                   skos:prefLabel "Break Down Value"@en .


###  http://www.fortiss.org/diprolea/ontosustain/rso#ConsumedEnergy
rso:ConsumedEnergy rdf:type owl:Class ;
                   rdfs:subClassOf rso:EnergyVariable ;
                   rdfs:comment "Variables (measurement objects) regarding consumed energy."@en ;
                   rdfs:label "Consumed Energy"@en ;
                   skos:prefLabel "Consumed Energy"@en .


###  http://www.fortiss.org/diprolea/ontosustain/rso#ConsumedEnergyIndicator
rso:ConsumedEnergyIndicator rdf:type owl:Class ;
                            owl:equivalentClass [ owl:intersectionOf ( rso:EnergyIndicator
                                                                       [ rdf:type owl:Restriction ;
                                                                         owl:onProperty rso:hasMeasurementVariable ;
                                                                         owl:someValuesFrom rso:ConsumedEnergy
                                                                       ]
                                                                     ) ;
                                                  rdf:type owl:Class
                                                ] ;
                            rdfs:comment "Indicator that measures the consumed energy subtopic."@en ;
                            rdfs:label "Consumed Energy Indicator"@en ;
                            skos:prefLabel "Consumed Energy Indicator"@en .


###  http://www.fortiss.org/diprolea/ontosustain/rso#ConsumedPurchasedCooling
rso:ConsumedPurchasedCooling rdf:type owl:Class ;
                             rdfs:subClassOf rso:ConsumedPurchasedSecondaryEnergy ;
                             rdfs:comment "Variables (measurement objects) regarding consumed purchased cooling."@en ;
                             rdfs:label "Consumed Purchased Cooling"@en ;
                             skos:prefLabel "Consumed Purchased Cooling"@en .


###  http://www.fortiss.org/diprolea/ontosustain/rso#ConsumedPurchasedCoolingFromNonRenewableSource
rso:ConsumedPurchasedCoolingFromNonRenewableSource rdf:type owl:Class ;
                                                   rdfs:subClassOf rso:ConsumedPurchasedCooling ;
                                                   owl:disjointWith rso:ConsumedPurchasedCoolingFromRenewableSource ;
                                                   rdfs:comment "Variables (measurement objects) regarding consumed purchased cooling from non-renewable sources."@en ;
                                                   rdfs:label "Consumed Purchased Cooling From Non-Renewable Source"@en ;
                                                   skos:prefLabel "Consumed Purchased Cooling From Non-Renewable Source"@en .


###  http://www.fortiss.org/diprolea/ontosustain/rso#ConsumedPurchasedCoolingFromNonRenewableSourceIndicator
rso:ConsumedPurchasedCoolingFromNonRenewableSourceIndicator rdf:type owl:Class ;
                                                            owl:equivalentClass [ owl:intersectionOf ( rso:ConsumedPurchasedCoolingIndicator
                                                                                                       [ rdf:type owl:Restriction ;
                                                                                                         owl:onProperty rso:hasMeasurementVariable ;
                                                                                                         owl:someValuesFrom rso:ConsumedPurchasedCoolingFromNonRenewableSource
                                                                                                       ]
                                                                                                     ) ;
                                                                                  rdf:type owl:Class
                                                                                ] ;
                                                            rdfs:comment "Indicator that measures the consumed purchased cooling from non-renewable source subtopic."@en ;
                                                            rdfs:label "Consumed Purchased Cooling From Non-Renewable Source Indicator"@en ;
                                                            skos:prefLabel "Consumed Purchased Cooling From Non-Renewable Source Indicator"@en .


###  http://www.fortiss.org/diprolea/ontosustain/rso#ConsumedPurchasedCoolingFromRenewableSource
rso:ConsumedPurchasedCoolingFromRenewableSource rdf:type owl:Class ;
                                                rdfs:subClassOf rso:ConsumedPurchasedCooling ;
                                                rdfs:comment "Variables (measurement objects) regarding consumed purchased cooling from renewable sources."@en ;
                                                rdfs:label "Consumed Purchased Cooling From Renewable Source"@en ;
                                                skos:prefLabel "Consumed Purchased Cooling From Renewable Source"@en .


###  http://www.fortiss.org/diprolea/ontosustain/rso#ConsumedPurchasedCoolingFromRenewableSourceIndicator
rso:ConsumedPurchasedCoolingFromRenewableSourceIndicator rdf:type owl:Class ;
                                                         owl:equivalentClass [ owl:intersectionOf ( rso:ConsumedPurchasedCoolingIndicator
                                                                                                    [ rdf:type owl:Restriction ;
                                                                                                      owl:onProperty rso:hasMeasurementVariable ;
                                                                                                      owl:someValuesFrom rso:ConsumedPurchasedCoolingFromRenewableSource
                                                                                                    ]
                                                                                                  ) ;
                                                                               rdf:type owl:Class
                                                                             ] ;
                                                         rdfs:comment "Indicator that measures the consumed purchased cooling from renewable source subtopic."@en ;
                                                         rdfs:label "Consumed Purchased Cooling From Renewable Source Indicator"@en ;
                                                         skos:prefLabel "Consumed Purchased Cooling From Renewable Source Indicator"@en .


###  http://www.fortiss.org/diprolea/ontosustain/rso#ConsumedPurchasedCoolingIndicator
rso:ConsumedPurchasedCoolingIndicator rdf:type owl:Class ;
                                      owl:equivalentClass [ owl:intersectionOf ( rso:ConsumedPurchasedSecondaryEnergyIndicator
                                                                                 [ rdf:type owl:Restriction ;
                                                                                   owl:onProperty rso:hasMeasurementVariable ;
                                                                                   owl:someValuesFrom rso:ConsumedPurchasedCooling
                                                                                 ]
                                                                               ) ;
                                                            rdf:type owl:Class
                                                          ] ;
                                      rdfs:comment "Indicator that measures the consumed purchased cooling subtopic."@en ;
                                      rdfs:label "Consumed Purchased Cooling Indicator"@en ;
                                      skos:prefLabel "Consumed Purchased Cooling Indicator"@en .


###  http://www.fortiss.org/diprolea/ontosustain/rso#ConsumedPurchasedElectricity
rso:ConsumedPurchasedElectricity rdf:type owl:Class ;
                                 rdfs:subClassOf rso:ConsumedPurchasedSecondaryEnergy ;
                                 rdfs:comment "Variables (measurement objects) regarding consumed purchased electricity."@en ;
                                 rdfs:label "Consumed Purchased Electricity"@en ;
                                 skos:prefLabel "Consumed Purchased Electricity"@en .


###  http://www.fortiss.org/diprolea/ontosustain/rso#ConsumedPurchasedElectricityFromNonRenewableSource
rso:ConsumedPurchasedElectricityFromNonRenewableSource rdf:type owl:Class ;
                                                       rdfs:subClassOf rso:ConsumedPurchasedElectricity ;
                                                       owl:disjointWith rso:ConsumedPurchasedElectricityFromRenewableSource ;
                                                       rdfs:comment "Variables (measurement objects) regarding consumed purchased electricity from non-renewable sources."@en ;
                                                       rdfs:label "Consumed Purchased Electricity From Non-Renewable Source"@en ;
                                                       skos:prefLabel "Consumed Purchased Electricity From Non-Renewable Source"@en .


###  http://www.fortiss.org/diprolea/ontosustain/rso#ConsumedPurchasedElectricityFromNonRenewableSourceIndicator
rso:ConsumedPurchasedElectricityFromNonRenewableSourceIndicator rdf:type owl:Class ;
                                                                owl:equivalentClass [ owl:intersectionOf ( rso:ConsumedPurchasedElectricityIndicator
                                                                                                           [ rdf:type owl:Restriction ;
                                                                                                             owl:onProperty rso:hasMeasurementVariable ;
                                                                                                             owl:someValuesFrom rso:ConsumedPurchasedHeatingFromNonRenewableSource
                                                                                                           ]
                                                                                                         ) ;
                                                                                      rdf:type owl:Class
                                                                                    ] ;
                                                                rdfs:comment "Indicator that measures the consumed purchased electricity from non-renewable source subtopic."@en ;
                                                                rdfs:label "Consumed Purchased Electricity From Non-Renewable Source Indicator"@en ;
                                                                skos:prefLabel "Consumed Purchased Electricity From Non-Renewable Source Indicator"@en .


###  http://www.fortiss.org/diprolea/ontosustain/rso#ConsumedPurchasedElectricityFromRenewableSource
rso:ConsumedPurchasedElectricityFromRenewableSource rdf:type owl:Class ;
                                                    rdfs:subClassOf rso:ConsumedPurchasedElectricity ;
                                                    rdfs:comment "Variables (measurement objects) regarding consumed purchased electricity from renewable sources."@en ;
                                                    rdfs:label "Consumed Purchased Electricity From Renewable Source"@en ;
                                                    skos:prefLabel "Consumed Purchased Electricity From Renewable Source"@en .


###  http://www.fortiss.org/diprolea/ontosustain/rso#ConsumedPurchasedElectricityFromRenewableSourceIndicator
rso:ConsumedPurchasedElectricityFromRenewableSourceIndicator rdf:type owl:Class ;
                                                             owl:equivalentClass [ owl:intersectionOf ( rso:ConsumedPurchasedElectricityIndicator
                                                                                                        [ rdf:type owl:Restriction ;
                                                                                                          owl:onProperty rso:hasMeasurementVariable ;
                                                                                                          owl:someValuesFrom rso:ConsumedPurchasedElectricityFromRenewableSource
                                                                                                        ]
                                                                                                      ) ;
                                                                                   rdf:type owl:Class
                                                                                 ] ;
                                                             rdfs:comment "Indicator that measures the consumed purchased electricity from renewable source subtopic."@en ;
                                                             rdfs:label "Consumed Purchased Electricity From Renewable Source Indicator"@en ;
                                                             skos:prefLabel "Consumed Purchased Electricity From Renewable Source Indicator"@en .


###  http://www.fortiss.org/diprolea/ontosustain/rso#ConsumedPurchasedElectricityIndicator
rso:ConsumedPurchasedElectricityIndicator rdf:type owl:Class ;
                                          owl:equivalentClass [ owl:intersectionOf ( rso:ConsumedPurchasedSecondaryEnergyIndicator
                                                                                     [ rdf:type owl:Restriction ;
                                                                                       owl:onProperty rso:hasMeasurementVariable ;
                                                                                       owl:someValuesFrom rso:ConsumedPurchasedElectricity
                                                                                     ]
                                                                                   ) ;
                                                                rdf:type owl:Class
                                                              ] ;
                                          rdfs:comment "Indicator that measures the consumed from purchased electricity subtopic."@en ;
                                          rdfs:label "Consumed Purchased Electricity Indicator"@en ;
                                          skos:prefLabel "Consumed Purchased Electricity Indicator"@en .


###  http://www.fortiss.org/diprolea/ontosustain/rso#ConsumedPurchasedEnergy
rso:ConsumedPurchasedEnergy rdf:type owl:Class ;
                            rdfs:subClassOf rso:ConsumedEnergy ;
                            rdfs:comment "Variables (measurement objects) regarding consumed purchased energy."@en ;
                            rdfs:label "Consumed Purchased Energy"@en ;
                            skos:prefLabel "Consumed Purchased Energy"@en .


###  http://www.fortiss.org/diprolea/ontosustain/rso#ConsumedPurchasedEnergyIndicator
rso:ConsumedPurchasedEnergyIndicator rdf:type owl:Class ;
                                     owl:equivalentClass [ owl:intersectionOf ( rso:ConsumedEnergyIndicator
                                                                                [ rdf:type owl:Restriction ;
                                                                                  owl:onProperty rso:hasMeasurementVariable ;
                                                                                  owl:someValuesFrom rso:ConsumedPurchasedEnergy
                                                                                ]
                                                                              ) ;
                                                           rdf:type owl:Class
                                                         ] ;
                                     rdfs:comment "Indicator that measures the consumed from purchased energy subtopic."@en ;
                                     rdfs:label "Consumed Purchased Energy Indicator"@en ;
                                     skos:prefLabel "Consumed Purchased Energy Indicator"@en .


###  http://www.fortiss.org/diprolea/ontosustain/rso#ConsumedPurchasedFuel
rso:ConsumedPurchasedFuel rdf:type owl:Class ;
                          rdfs:subClassOf rso:ConsumedPurchasedEnergy ;
                          owl:disjointWith rso:ConsumedPurchasedSecondaryEnergy ;
                          rdfs:comment "Variables (measurement objects) regarding consumed purchased first-level energy (fuel)."@en ;
                          rdfs:label "Consumed Purchased Fuel"@en ;
                          skos:prefLabel "Consumed Purchased Fuel"@en .


###  http://www.fortiss.org/diprolea/ontosustain/rso#ConsumedPurchasedFuelFromBiomass
rso:ConsumedPurchasedFuelFromBiomass rdf:type owl:Class ;
                                     rdfs:subClassOf rso:ConsumedPurchasedFuelFromRenewableSource ;
                                     rdfs:comment "Variables (measurement objects) regarding consumed purchased fuel from biomass."@en ;
                                     rdfs:label "Consumed Purchased Fuel From Biomass"@en ;
                                     skos:prefLabel "Consumed Purchased Fuel From Biomass"@en .


###  http://www.fortiss.org/diprolea/ontosustain/rso#ConsumedPurchasedFuelFromBiomassIndicator
rso:ConsumedPurchasedFuelFromBiomassIndicator rdf:type owl:Class ;
                                              owl:equivalentClass [ owl:intersectionOf ( rso:ConsumedPurchasedFuelFromRenewableSourceIndicator
                                                                                         [ rdf:type owl:Restriction ;
                                                                                           owl:onProperty rso:hasMeasurementVariable ;
                                                                                           owl:someValuesFrom rso:ConsumedPurchasedFuelFromBiomass
                                                                                         ]
                                                                                       ) ;
                                                                    rdf:type owl:Class
                                                                  ] ;
                                              rdfs:comment "Indicator that measures the consumed from purchased fuel from biomass subtopic."@en ;
                                              rdfs:label "Consumed Purchased Fuel From Biomass Indicator"@en ;
                                              skos:prefLabel "Consumed Purchased Fuel From Biomass Indicator"@en .


###  http://www.fortiss.org/diprolea/ontosustain/rso#ConsumedPurchasedFuelFromCoalAndCoalProduct
rso:ConsumedPurchasedFuelFromCoalAndCoalProduct rdf:type owl:Class ;
                                                rdfs:subClassOf rso:ConsumedPurchasedFuelFromNonRenewableSource ;
                                                rdfs:comment "Variables (measurement objects) regarding consumed purchased fuel from coal and coal product."@en ;
                                                rdfs:label "Consumed Purchased Fuel From Coal And Coal Product"@en ;
                                                skos:prefLabel "Consumed Purchased Fuel From Coal And Coal Product"@en .


###  http://www.fortiss.org/diprolea/ontosustain/rso#ConsumedPurchasedFuelFromCoalAndCoalProductIndicator
rso:ConsumedPurchasedFuelFromCoalAndCoalProductIndicator rdf:type owl:Class ;
                                                         owl:equivalentClass [ owl:intersectionOf ( rso:ConsumedPurchasedFuelFromNonRenewableSourceIndicator
                                                                                                    [ rdf:type owl:Restriction ;
                                                                                                      owl:onProperty rso:hasMeasurementVariable ;
                                                                                                      owl:someValuesFrom rso:ConsumedPurchasedFuelFromCoalAndCoalProduct
                                                                                                    ]
                                                                                                  ) ;
                                                                               rdf:type owl:Class
                                                                             ] ;
                                                         rdfs:comment "Indicator that measures the consumed from purchased fuel from coal and coal products subtopic."@en ;
                                                         rdfs:label "Consumed Purchased Fuel From Coal And Coal Product Indicator"@en ;
                                                         skos:prefLabel "Consumed Purchased Fuel From Coal And Coal Product Indicator"@en .


###  http://www.fortiss.org/diprolea/ontosustain/rso#ConsumedPurchasedFuelFromCrudeOilAndPetroleumProducts
rso:ConsumedPurchasedFuelFromCrudeOilAndPetroleumProducts rdf:type owl:Class ;
                                                          rdfs:subClassOf rso:ConsumedPurchasedFuelFromNonRenewableSource ;
                                                          rdfs:comment "Variables (measurement objects) regarding consumed purchased fuel from crude oil and petroleum products."@en ;
                                                          rdfs:label "Consumed Purchased Fuel From Crude Oil And Petroleum Products"@en ;
                                                          skos:prefLabel "Consumed Purchased Fuel From Crude Oil And Petroleum Products"@en .


###  http://www.fortiss.org/diprolea/ontosustain/rso#ConsumedPurchasedFuelFromCrudeOilAndPetroleumProductsIndicator
rso:ConsumedPurchasedFuelFromCrudeOilAndPetroleumProductsIndicator rdf:type owl:Class ;
                                                                   owl:equivalentClass [ owl:intersectionOf ( rso:ConsumedPurchasedFuelFromNonRenewableSourceIndicator
                                                                                                              [ rdf:type owl:Restriction ;
                                                                                                                owl:onProperty rso:hasMeasurementVariable ;
                                                                                                                owl:someValuesFrom rso:ConsumedPurchasedFuelFromCrudeOilAndPetroleumProducts
                                                                                                              ]
                                                                                                            ) ;
                                                                                         rdf:type owl:Class
                                                                                       ] ;
                                                                   rdfs:comment "Indicator that measures the consumed from purchased fuel from crude oil and petroleum products subtopic."@en ;
                                                                   rdfs:label "Consumed Purchased Fuel From Crude Oil And Petroleum Products Indicator"@en ;
                                                                   skos:prefLabel "Consumed Purchased Fuel From Crude Oil And Petroleum Products Indicator"@en .


###  http://www.fortiss.org/diprolea/ontosustain/rso#ConsumedPurchasedFuelFromGeothermal
rso:ConsumedPurchasedFuelFromGeothermal rdf:type owl:Class ;
                                        rdfs:subClassOf rso:ConsumedPurchasedFuelFromRenewableSource ;
                                        rdfs:comment "Variables (measurement objects) regarding consumed purchased fuel from geothermal."@en ;
                                        rdfs:label "Consumed Purchased Fuel From Geothermal"@en ;
                                        skos:prefLabel "Consumed Purchased Fuel From Geothermal"@en .


###  http://www.fortiss.org/diprolea/ontosustain/rso#ConsumedPurchasedFuelFromGeothermalIndicator
rso:ConsumedPurchasedFuelFromGeothermalIndicator rdf:type owl:Class ;
                                                 owl:equivalentClass [ owl:intersectionOf ( rso:ConsumedPurchasedFuelFromRenewableSourceIndicator
                                                                                            [ rdf:type owl:Restriction ;
                                                                                              owl:onProperty rso:hasMeasurementVariable ;
                                                                                              owl:someValuesFrom rso:ConsumedPurchasedFuelFromGeothermal
                                                                                            ]
                                                                                          ) ;
                                                                       rdf:type owl:Class
                                                                     ] ;
                                                 rdfs:comment "Indicator that measures the consumed from purchased fuel from geothermal subtopic."@en ;
                                                 rdfs:label "Consumed Purchased Fuel From Geothermal Indicator"@en ;
                                                 skos:prefLabel "Consumed Purchased Fuel From Geothermal Indicator"@en .


###  http://www.fortiss.org/diprolea/ontosustain/rso#ConsumedPurchasedFuelFromHydro
rso:ConsumedPurchasedFuelFromHydro rdf:type owl:Class ;
                                   rdfs:subClassOf rso:ConsumedPurchasedFuelFromRenewableSource ;
                                   rdfs:comment "Variables (measurement objects) regarding consumed purchased fuel from hydro."@en ;
                                   rdfs:label "Consumed Purchased Fuel From Hydro"@en ;
                                   skos:prefLabel "Consumed Purchased Fuel From Hydro"@en .


###  http://www.fortiss.org/diprolea/ontosustain/rso#ConsumedPurchasedFuelFromHydroIndicator
rso:ConsumedPurchasedFuelFromHydroIndicator rdf:type owl:Class ;
                                            owl:equivalentClass [ owl:intersectionOf ( rso:ConsumedPurchasedFuelFromRenewableSourceIndicator
                                                                                       [ rdf:type owl:Restriction ;
                                                                                         owl:onProperty rso:hasMeasurementVariable ;
                                                                                         owl:someValuesFrom rso:ConsumedPurchasedFuelFromHydro
                                                                                       ]
                                                                                     ) ;
                                                                  rdf:type owl:Class
                                                                ] ;
                                            rdfs:comment "Indicator that measures the consumed from purchased fuel from hydro subtopic."@en ;
                                            rdfs:label "Consumed Purchased Fuel From Hydro Indicator"@en ;
                                            skos:prefLabel "Consumed Purchased Fuel From Hydro Indicator"@en .


###  http://www.fortiss.org/diprolea/ontosustain/rso#ConsumedPurchasedFuelFromNaturalGas
rso:ConsumedPurchasedFuelFromNaturalGas rdf:type owl:Class ;
                                        rdfs:subClassOf rso:ConsumedPurchasedFuelFromNonRenewableSource ;
                                        rdfs:comment "Variables (measurement objects) regarding consumed purchased fuel from natural gas."@en ;
                                        rdfs:label "Consumed Purchased Fuel From Natural Gas"@en ;
                                        skos:prefLabel "Consumed Purchased Fuel From Natural Gas"@en .


###  http://www.fortiss.org/diprolea/ontosustain/rso#ConsumedPurchasedFuelFromNaturalGasIndicator
rso:ConsumedPurchasedFuelFromNaturalGasIndicator rdf:type owl:Class ;
                                                 owl:equivalentClass [ owl:intersectionOf ( rso:ConsumedPurchasedFuelFromNonRenewableSourceIndicator
                                                                                            [ rdf:type owl:Restriction ;
                                                                                              owl:onProperty rso:hasMeasurementVariable ;
                                                                                              owl:someValuesFrom rso:ConsumedPurchasedFuelFromNaturalGas
                                                                                            ]
                                                                                          ) ;
                                                                       rdf:type owl:Class
                                                                     ] ;
                                                 rdfs:comment "Indicator that measures the consumed from purchased fuel natural gas subtopic."@en ;
                                                 rdfs:label "Consumed Purchased Fuel From Natural Gas Indicator"@en ;
                                                 skos:prefLabel "Consumed Purchased Fuel From Natural Gas Indicator"@en .


###  http://www.fortiss.org/diprolea/ontosustain/rso#ConsumedPurchasedFuelFromNonRenewableSource
rso:ConsumedPurchasedFuelFromNonRenewableSource rdf:type owl:Class ;
                                                rdfs:subClassOf rso:ConsumedPurchasedFuel ;
                                                owl:disjointWith rso:ConsumedPurchasedFuelFromRenewableSource ;
                                                rdfs:comment "Variables (measurement objects) regarding consumed purchased fuel from non-renewable source, which refers to energy source that cannot be replenished, reproduced, grown or generated in a short time period through ecological cycles or agricultural processes."@en ;
                                                rdfs:label "Consumed Purchased Fuel From Non-Renewable Source"@en ;
                                                skos:prefLabel "Consumed Purchased Fuel From Non-Renewable Source"@en .


###  http://www.fortiss.org/diprolea/ontosustain/rso#ConsumedPurchasedFuelFromNonRenewableSourceIndicator
rso:ConsumedPurchasedFuelFromNonRenewableSourceIndicator rdf:type owl:Class ;
                                                         owl:equivalentClass [ owl:intersectionOf ( rso:ConsumedPurchasedFuelIndicator
                                                                                                    [ rdf:type owl:Restriction ;
                                                                                                      owl:onProperty rso:hasMeasurementVariable ;
                                                                                                      owl:someValuesFrom rso:ConsumedPurchasedFuelFromNonRenewableSource
                                                                                                    ]
                                                                                                  ) ;
                                                                               rdf:type owl:Class
                                                                             ] ;
                                                         rdfs:comment "Indicator that measures the consumed from purchased fuel from non-renewable sources subtopic."@en ;
                                                         rdfs:label "Consumed Purchased Fuel From Non-Renewable Source Indicator"@en ;
                                                         skos:prefLabel "Consumed Purchased Fuel From Non-Renewable Source Indicator"@en .


###  http://www.fortiss.org/diprolea/ontosustain/rso#ConsumedPurchasedFuelFromNuclearProduct
rso:ConsumedPurchasedFuelFromNuclearProduct rdf:type owl:Class ;
                                            rdfs:subClassOf rso:ConsumedPurchasedFuelFromNonRenewableSource ;
                                            rdfs:comment "Variables (measurement objects) regarding consumed purchased fuel from nuclear product."@en ;
                                            rdfs:label "Consumed Purchased Fuel From Nuclear Product"@en ;
                                            skos:prefLabel "Consumed Purchased Fuel From Nuclear Product"@en .


###  http://www.fortiss.org/diprolea/ontosustain/rso#ConsumedPurchasedFuelFromNuclearProductIndicator
rso:ConsumedPurchasedFuelFromNuclearProductIndicator rdf:type owl:Class ;
                                                     owl:equivalentClass [ owl:intersectionOf ( rso:ConsumedPurchasedFuelFromNonRenewableSourceIndicator
                                                                                                [ rdf:type owl:Restriction ;
                                                                                                  owl:onProperty rso:hasMeasurementVariable ;
                                                                                                  owl:someValuesFrom rso:ConsumedPurchasedFuelFromNuclearProduct
                                                                                                ]
                                                                                              ) ;
                                                                           rdf:type owl:Class
                                                                         ] ;
                                                     rdfs:comment "Indicator that measures the consumed from purchased nuclear products subtopic."@en ;
                                                     rdfs:label "Consumed Purchased Fuel From Nuclear Product Indicator"@en ;
                                                     skos:prefLabel "Consumed Purchased Fuel From Nuclear Product Indicator"@en .


###  http://www.fortiss.org/diprolea/ontosustain/rso#ConsumedPurchasedFuelFromOtherNon-renewableSources
rso:ConsumedPurchasedFuelFromOtherNon-renewableSources rdf:type owl:Class ;
                                                       rdfs:subClassOf rso:ConsumedPurchasedFuelFromNonRenewableSource ;
                                                       rdfs:comment "Variables (measurement objects) regarding consumed purchased fuel from other non-renewable sources."@en ;
                                                       rdfs:label "Consumed Purchased Fuel From Other Non-renewable Sources"@en ;
                                                       skos:prefLabel "Consumed Purchased Fuel From Other Non-renewable Sources"@en .


###  http://www.fortiss.org/diprolea/ontosustain/rso#ConsumedPurchasedFuelFromOtherNon-renewableSourcesIndicator
rso:ConsumedPurchasedFuelFromOtherNon-renewableSourcesIndicator rdf:type owl:Class ;
                                                                owl:equivalentClass [ owl:intersectionOf ( rso:ConsumedPurchasedFuelFromNonRenewableSourceIndicator
                                                                                                           [ rdf:type owl:Restriction ;
                                                                                                             owl:onProperty rso:hasMeasurementVariable ;
                                                                                                             owl:someValuesFrom rso:ConsumedPurchasedFuelFromOtherNon-renewableSources
                                                                                                           ]
                                                                                                         ) ;
                                                                                      rdf:type owl:Class
                                                                                    ] ;
                                                                rdfs:comment "Indicator that measures the consumed from other non-renewable sources subtopic."@en ;
                                                                rdfs:label "Consumed Purchased Fuel From Other Non-renewable Sources Indicator"@en ;
                                                                skos:prefLabel "Consumed Purchased Fuel From Other Non-renewable Sources Indicator"@en .


###  http://www.fortiss.org/diprolea/ontosustain/rso#ConsumedPurchasedFuelFromRenewableSource
rso:ConsumedPurchasedFuelFromRenewableSource rdf:type owl:Class ;
                                             rdfs:subClassOf rso:ConsumedPurchasedFuel ;
                                             rdfs:comment "Variables (measurement objects) regarding consumed purchased fuel from renewable source, which refers to energy source that is capable of being replenished in a short time through ecological cycles or agricultural processes."@en ;
                                             rdfs:label "Consumed Purchased Fuel From Renewable Source"@en ;
                                             skos:prefLabel "Consumed Purchased Fuel From Renewable Source"@en .


###  http://www.fortiss.org/diprolea/ontosustain/rso#ConsumedPurchasedFuelFromRenewableSourceIndicator
rso:ConsumedPurchasedFuelFromRenewableSourceIndicator rdf:type owl:Class ;
                                                      owl:equivalentClass [ owl:intersectionOf ( rso:ConsumedPurchasedFuelIndicator
                                                                                                 [ rdf:type owl:Restriction ;
                                                                                                   owl:onProperty rso:hasMeasurementVariable ;
                                                                                                   owl:someValuesFrom rso:ConsumedPurchasedFuelFromRenewableSource
                                                                                                 ]
                                                                                               ) ;
                                                                            rdf:type owl:Class
                                                                          ] ;
                                                      rdfs:comment "Indicator that measures the consumed from purchased fuel from renewable sources subtopic."@en ;
                                                      rdfs:label "Consumed Purchased Fuel From Renewable Source Indicator"@en ;
                                                      skos:prefLabel "Consumed Purchased Fuel From Renewable Source Indicator"@en .


###  http://www.fortiss.org/diprolea/ontosustain/rso#ConsumedPurchasedFuelFromSolar
rso:ConsumedPurchasedFuelFromSolar rdf:type owl:Class ;
                                   rdfs:subClassOf rso:ConsumedPurchasedFuelFromRenewableSource ;
                                   rdfs:comment "Variables (measurement objects) regarding consumed purchased fuel from solar."@en ;
                                   rdfs:label "Consumed Purchased Fuel From Solar"@en ;
                                   skos:prefLabel "Consumed Purchased Fuel From Solar"@en .


###  http://www.fortiss.org/diprolea/ontosustain/rso#ConsumedPurchasedFuelFromSolarIndicator
rso:ConsumedPurchasedFuelFromSolarIndicator rdf:type owl:Class ;
                                            owl:equivalentClass [ owl:intersectionOf ( rso:ConsumedPurchasedFuelFromRenewableSourceIndicator
                                                                                       [ rdf:type owl:Restriction ;
                                                                                         owl:onProperty rso:hasMeasurementVariable ;
                                                                                         owl:someValuesFrom rso:ConsumedPurchasedFuelFromSolar
                                                                                       ]
                                                                                     ) ;
                                                                  rdf:type owl:Class
                                                                ] ;
                                            rdfs:comment "Indicator that measures the consumed from purchased fuel from solar subtopic."@en ;
                                            rdfs:label "Consumed Purchased Fuel From Solar Indicator"@en ;
                                            skos:prefLabel "Consumed Purchased Fuel From Solar Indicator"@en .


###  http://www.fortiss.org/diprolea/ontosustain/rso#ConsumedPurchasedFuelFromWind
rso:ConsumedPurchasedFuelFromWind rdf:type owl:Class ;
                                  rdfs:subClassOf rso:ConsumedPurchasedFuelFromRenewableSource ;
                                  rdfs:comment "Variables (measurement objects) regarding consumed purchased fuel from wind."@en ;
                                  rdfs:label "Consumed Purchased Fuel From Wind"@en ;
                                  skos:prefLabel "Consumed Purchased Fuel From Wind"@en .


###  http://www.fortiss.org/diprolea/ontosustain/rso#ConsumedPurchasedFuelFromWindIndicator
rso:ConsumedPurchasedFuelFromWindIndicator rdf:type owl:Class ;
                                           owl:equivalentClass [ owl:intersectionOf ( rso:ConsumedPurchasedFuelFromRenewableSourceIndicator
                                                                                      [ rdf:type owl:Restriction ;
                                                                                        owl:onProperty rso:hasMeasurementVariable ;
                                                                                        owl:someValuesFrom rso:ConsumedPurchasedFuelFromWind
                                                                                      ]
                                                                                    ) ;
                                                                 rdf:type owl:Class
                                                               ] ;
                                           rdfs:comment "Indicator that measures the consumed from purchased fuel from wind subtopic."@en ;
                                           rdfs:label "Consumed Purchased Fuel From Wind Indicator"@en ;
                                           skos:prefLabel "Consumed Purchased Fuel From Wind Indicator"@en .


###  http://www.fortiss.org/diprolea/ontosustain/rso#ConsumedPurchasedFuelIndicator
rso:ConsumedPurchasedFuelIndicator rdf:type owl:Class ;
                                   owl:equivalentClass [ owl:intersectionOf ( rso:ConsumedPurchasedEnergyIndicator
                                                                              [ rdf:type owl:Restriction ;
                                                                                owl:onProperty rso:hasMeasurementVariable ;
                                                                                owl:someValuesFrom rso:ConsumedPurchasedFuel
                                                                              ]
                                                                            ) ;
                                                         rdf:type owl:Class
                                                       ] ;
                                   rdfs:comment "Indicator that measures the consumed from purchased fuel (first-level energy) subtopic."@en ;
                                   rdfs:label "Consumed Purchased Fuel Indicator"@en ;
                                   skos:prefLabel "Consumed Purchased Fuel Indicator"@en .


###  http://www.fortiss.org/diprolea/ontosustain/rso#ConsumedPurchasedHeating
rso:ConsumedPurchasedHeating rdf:type owl:Class ;
                             rdfs:subClassOf rso:ConsumedPurchasedSecondaryEnergy ;
                             rdfs:comment "Variables (measurement objects) regarding consumed purchased heating."@en ;
                             rdfs:label "Consumed Purchased Heating"@en ;
                             skos:prefLabel "Consumed Purchased Heating"@en .


###  http://www.fortiss.org/diprolea/ontosustain/rso#ConsumedPurchasedHeatingFromNonRenewableSource
rso:ConsumedPurchasedHeatingFromNonRenewableSource rdf:type owl:Class ;
                                                   rdfs:subClassOf rso:ConsumedPurchasedHeating ;
                                                   owl:disjointWith rso:ConsumedPurchasedHeatingFromRenewableSource ;
                                                   rdfs:comment "Variables (measurement objects) regarding consumed purchased heating from non-renewable sources."@en ;
                                                   rdfs:label "Consumed Purchased Heating From Non-Renewable Source"@en ;
                                                   skos:prefLabel "Consumed Purchased Heating From Non-Renewable Source"@en .


###  http://www.fortiss.org/diprolea/ontosustain/rso#ConsumedPurchasedHeatingFromNonRenewableSourceIndicator
rso:ConsumedPurchasedHeatingFromNonRenewableSourceIndicator rdf:type owl:Class ;
                                                            owl:equivalentClass [ owl:intersectionOf ( rso:ConsumedPurchasedHeatingIndicator
                                                                                                       [ rdf:type owl:Restriction ;
                                                                                                         owl:onProperty rso:hasMeasurementVariable ;
                                                                                                         owl:someValuesFrom rso:ConsumedPurchasedHeatingFromNonRenewableSource
                                                                                                       ]
                                                                                                     ) ;
                                                                                  rdf:type owl:Class
                                                                                ] ;
                                                            rdfs:comment "Indicator that measures the consumed purchased heating from non-renewable source subtopic."@en ;
                                                            rdfs:label "Consumed Purchased Heating From Non-Renewable Source Indicator"@en ;
                                                            skos:prefLabel "Consumed Purchased Heating From Non-Renewable Source Indicator"@en .


###  http://www.fortiss.org/diprolea/ontosustain/rso#ConsumedPurchasedHeatingFromRenewableSource
rso:ConsumedPurchasedHeatingFromRenewableSource rdf:type owl:Class ;
                                                rdfs:subClassOf rso:ConsumedPurchasedHeating ;
                                                rdfs:comment "Variables (measurement objects) regarding consumed purchased heating from renewable sources."@en ;
                                                rdfs:label "Consumed Purchased Heating From Renewable Source"@en ;
                                                skos:prefLabel "Consumed Purchased Heating From Renewable Source"@en .


###  http://www.fortiss.org/diprolea/ontosustain/rso#ConsumedPurchasedHeatingFromRenewableSourceIndicator
rso:ConsumedPurchasedHeatingFromRenewableSourceIndicator rdf:type owl:Class ;
                                                         owl:equivalentClass [ owl:intersectionOf ( rso:ConsumedPurchasedHeatingIndicator
                                                                                                    [ rdf:type owl:Restriction ;
                                                                                                      owl:onProperty rso:hasMeasurementVariable ;
                                                                                                      owl:someValuesFrom rso:ConsumedPurchasedHeatingFromRenewableSource
                                                                                                    ]
                                                                                                  ) ;
                                                                               rdf:type owl:Class
                                                                             ] ;
                                                         rdfs:comment "Indicator that measures the consumed purchased heating from renewable source subtopic."@en ;
                                                         rdfs:label "Consumed Purchased Heating From Renewable Source Indicator"@en ;
                                                         skos:prefLabel "Consumed Purchased Heating From Renewable Source Indicator"@en .


###  http://www.fortiss.org/diprolea/ontosustain/rso#ConsumedPurchasedHeatingIndicator
rso:ConsumedPurchasedHeatingIndicator rdf:type owl:Class ;
                                      owl:equivalentClass [ owl:intersectionOf ( rso:ConsumedPurchasedSecondaryEnergyIndicator
                                                                                 [ rdf:type owl:Restriction ;
                                                                                   owl:onProperty rso:hasMeasurementVariable ;
                                                                                   owl:someValuesFrom rso:ConsumedPurchasedHeating
                                                                                 ]
                                                                               ) ;
                                                            rdf:type owl:Class
                                                          ] ;
                                      rdfs:comment "Indicator that measures the consumed from purchased heating subtopic."@en ;
                                      rdfs:label "Consumed Purchased Heating Indicator"@en ;
                                      skos:prefLabel "Consumed Purchased Heating Indicator"@en .


###  http://www.fortiss.org/diprolea/ontosustain/rso#ConsumedPurchasedSecondaryEnergy
rso:ConsumedPurchasedSecondaryEnergy rdf:type owl:Class ;
                                     rdfs:subClassOf rso:ConsumedPurchasedEnergy ;
                                     rdfs:comment "Variables (measurement objects) regarding consumed purchased secondary energy."@en ;
                                     rdfs:label "Consumed Purchased Secondary Energy"@en ;
                                     skos:prefLabel "Consumed Purchased Secondary Energy"@en .


###  http://www.fortiss.org/diprolea/ontosustain/rso#ConsumedPurchasedSecondaryEnergyIndicator
rso:ConsumedPurchasedSecondaryEnergyIndicator rdf:type owl:Class ;
                                              owl:equivalentClass [ owl:intersectionOf ( rso:ConsumedPurchasedEnergyIndicator
                                                                                         [ rdf:type owl:Restriction ;
                                                                                           owl:onProperty rso:hasMeasurementVariable ;
                                                                                           owl:someValuesFrom rso:ConsumedPurchasedSecondaryEnergy
                                                                                         ]
                                                                                       ) ;
                                                                    rdf:type owl:Class
                                                                  ] ;
                                              rdfs:comment "Indicator that measures the consumed from purchased secondary energy subtopic."@en ;
                                              rdfs:label "Consumed Purchased Secondary Energy Indicator"@en ;
                                              skos:prefLabel "Consumed Purchased Secondary Energy Indicator"@en .


###  http://www.fortiss.org/diprolea/ontosustain/rso#ConsumedPurchasedSteam
rso:ConsumedPurchasedSteam rdf:type owl:Class ;
                           rdfs:subClassOf rso:ConsumedPurchasedSecondaryEnergy ;
                           rdfs:comment "Variables (measurement objects) regarding consumed purchased steam."@en ;
                           rdfs:label "Consumed Purchased Steam"@en ;
                           skos:prefLabel "Consumed Purchased Steam"@en .


###  http://www.fortiss.org/diprolea/ontosustain/rso#ConsumedPurchasedSteamFromNonRenewableSource
rso:ConsumedPurchasedSteamFromNonRenewableSource rdf:type owl:Class ;
                                                 rdfs:subClassOf rso:ConsumedPurchasedSteam ;
                                                 owl:disjointWith rso:ConsumedPurchasedSteamFromRenewableSource ;
                                                 rdfs:comment "Variables (measurement objects) regarding consumed purchased steam from non-renewable sources."@en ;
                                                 rdfs:label "Consumed Purchased Steam From Non-Renewable Source"@en ;
                                                 skos:prefLabel "Consumed Purchased Steam From Non-Renewable Source"@en .


###  http://www.fortiss.org/diprolea/ontosustain/rso#ConsumedPurchasedSteamFromNonRenewableSourceIndicator
rso:ConsumedPurchasedSteamFromNonRenewableSourceIndicator rdf:type owl:Class ;
                                                          owl:equivalentClass [ owl:intersectionOf ( rso:ConsumedPurchasedSteamIndicator
                                                                                                     [ rdf:type owl:Restriction ;
                                                                                                       owl:onProperty rso:hasMeasurementVariable ;
                                                                                                       owl:someValuesFrom rso:ConsumedPurchasedSteamFromNonRenewableSource
                                                                                                     ]
                                                                                                   ) ;
                                                                                rdf:type owl:Class
                                                                              ] ;
                                                          rdfs:comment "Indicator that measures the consumed purchased steam from non-renewable source subtopic."@en ;
                                                          rdfs:label "Consumed Purchased Steam From Non-Renewable Source Indicator"@en ;
                                                          skos:prefLabel "Consumed Purchased Steam From Non-Renewable Source Indicator"@en .


###  http://www.fortiss.org/diprolea/ontosustain/rso#ConsumedPurchasedSteamFromRenewableSource
rso:ConsumedPurchasedSteamFromRenewableSource rdf:type owl:Class ;
                                              rdfs:subClassOf rso:ConsumedPurchasedSteam ;
                                              rdfs:comment "Variables (measurement objects) regarding consumed purchased steam from renewable sources."@en ;
                                              rdfs:label "Consumed Purchased Steam From Renewable Source"@en ;
                                              skos:prefLabel "Consumed Purchased Steam From Renewable Source"@en .


###  http://www.fortiss.org/diprolea/ontosustain/rso#ConsumedPurchasedSteamFromRenewableSourceIndicator
rso:ConsumedPurchasedSteamFromRenewableSourceIndicator rdf:type owl:Class ;
                                                       owl:equivalentClass [ owl:intersectionOf ( rso:ConsumedPurchasedSteamIndicator
                                                                                                  [ rdf:type owl:Restriction ;
                                                                                                    owl:onProperty rso:hasMeasurementVariable ;
                                                                                                    owl:someValuesFrom rso:ConsumedPurchasedSteamFromRenewableSource
                                                                                                  ]
                                                                                                ) ;
                                                                             rdf:type owl:Class
                                                                           ] ;
                                                       rdfs:comment "Indicator that measures the consumed purchased steam from renewable source subtopic."@en ;
                                                       rdfs:label "Consumed Purchased Steam From Renewable Source Indicator"@en ;
                                                       skos:prefLabel "Consumed Purchased Steam From Renewable Source Indicator"@en .


###  http://www.fortiss.org/diprolea/ontosustain/rso#ConsumedPurchasedSteamIndicator
rso:ConsumedPurchasedSteamIndicator rdf:type owl:Class ;
                                    owl:equivalentClass [ owl:intersectionOf ( rso:ConsumedPurchasedSecondaryEnergyIndicator
                                                                               [ rdf:type owl:Restriction ;
                                                                                 owl:onProperty rso:hasMeasurementVariable ;
                                                                                 owl:someValuesFrom rso:ConsumedPurchasedSteam
                                                                               ]
                                                                             ) ;
                                                          rdf:type owl:Class
                                                        ] ;
                                    rdfs:comment "Indicator that measures the consumed from purchased steam subtopic."@en ;
                                    rdfs:label "Consumed Purchased Steam Indicator"@en ;
                                    skos:prefLabel "Consumed Purchased Steam Indicator"@en .


###  http://www.fortiss.org/diprolea/ontosustain/rso#ConsumedSelfGeneratedEnergy
rso:ConsumedSelfGeneratedEnergy rdf:type owl:Class ;
                                rdfs:subClassOf rso:ConsumedEnergy ;
                                rdfs:comment "Variables (measurement objects) regarding consumed self-generated energy"@en ;
                                rdfs:label "Consumed Self Generated Energy"@en ;
                                skos:prefLabel "Consumed Self Generated Energy"@en .


###  http://www.fortiss.org/diprolea/ontosustain/rso#ConsumedSelfGeneratedEnergyIndicator
rso:ConsumedSelfGeneratedEnergyIndicator rdf:type owl:Class ;
                                         owl:equivalentClass [ owl:intersectionOf ( rso:ConsumedEnergyIndicator
                                                                                    [ rdf:type owl:Restriction ;
                                                                                      owl:onProperty rso:hasMeasurementVariable ;
                                                                                      owl:someValuesFrom rso:ConsumedSelfGeneratedEnergy
                                                                                    ]
                                                                                  ) ;
                                                               rdf:type owl:Class
                                                             ] ;
                                         rdfs:comment "Indicator that measures the consumed from self generated energy subtopic."@en ;
                                         rdfs:label "Consumed Self Generated Energy Indicator"@en ;
                                         skos:prefLabel "Consumed Self Generated Energy Indicator"@en .


###  http://www.fortiss.org/diprolea/ontosustain/rso#CoreEnvironmentTopic
rso:CoreEnvironmentTopic rdf:type owl:Class ;
                         rdfs:subClassOf rso:CoreTopic ;
                         rdfs:comment "Individuals of CoreEnvironmentalTopic derive from the GRI standards and represent specific environmental issues. This classification aids in organizing and addressing distinct environmental aspects through targeted indicators."@en ;
                         rdfs:label "Core Environment Topic"@en ;
                         skos:prefLabel "Core Environment Topic"@en .


###  http://www.fortiss.org/diprolea/ontosustain/rso#CoreGovernanceTopic
rso:CoreGovernanceTopic rdf:type owl:Class ;
                        rdfs:subClassOf rso:CoreTopic ;
                        rdfs:comment "Individuals of CoreGovernanceTopic are based on the GRI standards and represent unique governance concerns. These topics facilitate the categorization of governance-related indicators, promoting transparency and accountability in corporate governance practices."@en ;
                        rdfs:label "Core Governance Topic"@en ;
                        skos:prefLabel "Core Governance Topic"@en .


###  http://www.fortiss.org/diprolea/ontosustain/rso#CoreSocialTopic
rso:CoreSocialTopic rdf:type owl:Class ;
                    rdfs:subClassOf rso:CoreTopic ;
                    rdfs:comment "Individuals of CoreSocialTopic are sourced from the GRI standards and encompass specific social issues. This categorization helps in the systematic reporting and evaluation of social topics, focusing on areas such as labor practices, human rights, and community engagement."@en ;
                    rdfs:label "Core Social Topic"@en ;
                    skos:prefLabel "Core Social Topic"@en .


###  http://www.fortiss.org/diprolea/ontosustain/rso#CoreTopic
rso:CoreTopic rdf:type owl:Class ;
              rdfs:subClassOf rso:Topic ;
              rdfs:comment "Individuals of CoreTopic are borrowed from the GRI standards which represents a singular environmental issue, facilitating indicator classification."@en ;
              rdfs:label "Core Topic"@en ;
              skos:prefLabel "Core Topic"@en .


###  http://www.fortiss.org/diprolea/ontosustain/rso#CorporateGovernanceIndicator
rso:CorporateGovernanceIndicator rdf:type owl:Class ;
                                 owl:equivalentClass [ owl:intersectionOf ( rso:Indicator
                                                                            [ rdf:type owl:Restriction ;
                                                                              owl:onProperty rso:measuresDimension ;
                                                                              owl:hasValue rso:Governance
                                                                            ]
                                                                          ) ;
                                                       rdf:type owl:Class
                                                     ] ;
                                 rdfs:comment "Indicators measure the corporate governance dimension of sustainability."@en ;
                                 rdfs:label "Corporate governance indicator"@en ;
                                 skos:prefLabel "Corporate governance indicator"@en .


###  http://www.fortiss.org/diprolea/ontosustain/rso#DirectGHGEmission
rso:DirectGHGEmission rdf:type owl:Class ;
                      rdfs:subClassOf rso:GHGEmission ;
                      owl:disjointWith rso:IndirectGHGEmission ;
                      rdfs:comment "Scope 1 GHG emissions, greenhouse gas (GHG) emissions from sources that are owned or controlled by the organization."@en ;
                      rdfs:isDefinedBy "https://www.globalreporting.org/publications/documents/english/gri-305-emissions-2016/" ;
                      rdfs:label "Direct GHG Emission"@en ;
                      skos:prefLabel "Direct GHG Emission"@en .


###  http://www.fortiss.org/diprolea/ontosustain/rso#DirectGHGEmissionIndicator
rso:DirectGHGEmissionIndicator rdf:type owl:Class ;
                               owl:equivalentClass [ owl:intersectionOf ( rso:GHGEmissionIndicator
                                                                          [ rdf:type owl:Restriction ;
                                                                            owl:onProperty rso:hasMeasurementVariable ;
                                                                            owl:someValuesFrom rso:DirectGHGEmission
                                                                          ]
                                                                        ) ;
                                                     rdf:type owl:Class
                                                   ] ;
                               owl:disjointWith rso:IndirectGHGEmissionIndicator ;
                               rdfs:comment "Indicator that measures the direct GHG (scope 1) emission subtopic."@en ;
                               rdfs:label "Direct GHG Emission Indicator" ;
                               skos:prefLabel "Direct GHG Emission Indicator" .


###  http://www.fortiss.org/diprolea/ontosustain/rso#Disclosure
rso:Disclosure rdf:type owl:Class ;
               rdfs:comment "Covers indicators that allow an organization to report information about sustainability issues. This class is further subdivided into GRIDisclosure and ESRSDisclosureRequirement based on terms used in each standard respectively."@en ;
               rdfs:label "Disclosure"@en ;
               skos:prefLabel "Disclosure"@en .


###  http://www.fortiss.org/diprolea/ontosustain/rso#ESGDimension
rso:ESGDimension rdf:type owl:Class ;
                 owl:equivalentClass [ rdf:type owl:Class ;
                                       owl:oneOf ( rso:Environment
                                                   rso:Governance
                                                   rso:Social
                                                 )
                                     ] ;
                 rdfs:comment "Covers the three dimensions of sustainability and is defined as enumerated class."@en ;
                 rdfs:label "ESG Dimension"@en ;
                 skos:prefLabel "ESG Dimension"@en .


###  http://www.fortiss.org/diprolea/ontosustain/rso#ESRSDisclosureRequirement
rso:ESRSDisclosureRequirement rdf:type owl:Class ;
                              rdfs:subClassOf rso:Disclosure ;
                              rdfs:comment """ESRS structure the information to be disclosed under Disclosure Requirements.
Disclosure Requirements consist of more granular datapoints. The term “datapoint” in this context also refers to a narrative sub-element of a Disclosure Requirement."""@en ;
                              rdfs:isDefinedBy "https://www.efrag.org/Assets/Download?assetUrl=%2Fsites%2Fwebpublishing%2FSiteAssets%2F06%2520Draft%2520ESRS%25201%2520General%2520requirements%2520November%25202022.pdf"^^xsd:anyURI ;
                              rdfs:label "ESRS Disclosure Requirement"@en ;
                              skos:definition """ESRS structure the information to be disclosed under Disclosure Requirements.
Disclosure Requirements consist of more granular datapoints. The term “datapoint” in this context also refers to a narrative sub-element of a Disclosure Requirement."""@en ;
                              skos:prefLabel "ESRS Disclosure Requirement"@en .


###  http://www.fortiss.org/diprolea/ontosustain/rso#ESRSEnvironmentTopic
rso:ESRSEnvironmentTopic rdf:type owl:Class ;
                         rdfs:subClassOf rso:ESRSTopic ;
                         rdfs:comment "ESRS topics derived from the ESRS standards describing the environmental dimension."@en ;
                         rdfs:label "ESRS Environment Topic"@en ;
                         skos:prefLabel "ESRS Environment Topic"@en .


###  http://www.fortiss.org/diprolea/ontosustain/rso#ESRSGovernanceTopic
rso:ESRSGovernanceTopic rdf:type owl:Class ;
                        rdfs:subClassOf rso:ESRSTopic ;
                        rdfs:comment "ESRS topics derived from the ESRS standards describing the governance dimension."@en ;
                        rdfs:label "ESRS Governance Topic"@en ;
                        skos:prefLabel "ESRS Governance Topic"@en .


###  http://www.fortiss.org/diprolea/ontosustain/rso#ESRSIndicator
rso:ESRSIndicator rdf:type owl:Class ;
                  rdfs:subClassOf rso:Indicator ;
                  owl:disjointWith rso:GRIIndicator ;
                  rdfs:comment "Indicators derived from the ESRS standards."@en ;
                  rdfs:label "ESRS Indicator"@en ;
                  skos:prefLabel "ESRS Indicator"@en .


###  http://www.fortiss.org/diprolea/ontosustain/rso#ESRSSocialTopic
rso:ESRSSocialTopic rdf:type owl:Class ;
                    rdfs:subClassOf rso:ESRSTopic ;
                    rdfs:comment "ESRS topics derived from the ESRS standards describing the social dimension."@en ;
                    rdfs:label "ESRS Social Topic"@en ;
                    skos:prefLabel "ESRS Social Topic"@en .


###  http://www.fortiss.org/diprolea/ontosustain/rso#ESRSStandard
rso:ESRSStandard rdf:type owl:Class ;
                 rdfs:subClassOf rso:Standard ;
                 rdfs:comment "A piece of the sustainability reporting standard derived from the ESRS."@en ;
                 rdfs:label "ESRS Standard"@en ;
                 skos:prefLabel "ESRS Standard"@en .


###  http://www.fortiss.org/diprolea/ontosustain/rso#ESRSTopic
rso:ESRSTopic rdf:type owl:Class ;
              rdfs:subClassOf rso:Topic ;
              rdfs:comment "ESRS topics derived from the ESRS standards."@en ;
              rdfs:label "ESRS Topic"@en ;
              skos:prefLabel "ESRS Topic"@en .


###  http://www.fortiss.org/diprolea/ontosustain/rso#ESRSTopicalStandard
rso:ESRSTopicalStandard rdf:type owl:Class ;
                        rdfs:subClassOf rso:ESRSStandard ;
                        owl:disjointWith rso:ESRSUniversalStandard ;
                        rdfs:comment "ESRS topical standards provide detailed disclosure requirements across environmental (E), social (S), and governance (G) topics. Environmental (E) topic focus on aspects related to environmental impact, such as climate change, biodiversity, and resource use. Social (S) standards address social matters, including human rights, labor practices, and community engagement.Governance (G) standards pertain to governance practices, board structures, and transparency."@en ;
                        rdfs:label "ESRS Topical Standard"@en ;
                        skos:prefLabel "ESRS Topical Standard"@en .


###  http://www.fortiss.org/diprolea/ontosustain/rso#ESRSUniversalStandard
rso:ESRSUniversalStandard rdf:type owl:Class ;
                          rdfs:subClassOf rso:ESRSStandard ;
                          rdfs:comment "ESRS universal standards provide general reporting concepts and overarching disclosure requirements that apply across all undertakings, regardless of the sector they operate in."@en ;
                          rdfs:label "ESRS Universal Standard"@en ;
                          skos:prefLabel "ESRS Universal Standard"@en .


###  http://www.fortiss.org/diprolea/ontosustain/rso#ElectricityIndirectGHGEmission
rso:ElectricityIndirectGHGEmission rdf:type owl:Class ;
                                   rdfs:subClassOf rso:IndirectGHGEmission ;
                                   owl:disjointWith rso:OtherIndirectGHGEmission ;
                                   rdfs:comment "Scope 2 GHG emissions, greenhouse gas (GHG) emissions that result from the generation of purchased or acquired electricity, heating, cooling, and steam consumed by the organization."@en ;
                                   rdfs:isDefinedBy "https://www.globalreporting.org/publications/documents/english/gri-305-emissions-2016/" ;
                                   rdfs:label "Electricity indirect GHG emission"@en ;
                                   skos:prefLabel "Electricity indirect GHG emission"@en .


###  http://www.fortiss.org/diprolea/ontosustain/rso#ElectricityIndirectGHGEmissionIndicator
rso:ElectricityIndirectGHGEmissionIndicator rdf:type owl:Class ;
                                            owl:equivalentClass [ owl:intersectionOf ( rso:IndirectGHGEmissionIndicator
                                                                                       [ rdf:type owl:Restriction ;
                                                                                         owl:onProperty rso:hasMeasurementVariable ;
                                                                                         owl:someValuesFrom rso:ElectricityIndirectGHGEmission
                                                                                       ]
                                                                                     ) ;
                                                                  rdf:type owl:Class
                                                                ] ;
                                            owl:disjointWith rso:OtherIndirectGHGEmissionIndicator ;
                                            rdfs:comment "Indicator that measures the electricity indirect GHG (scope 2) emission subtopic."@en ;
                                            rdfs:label "Electricity Indirect GHG Emission Indicator"@en ;
                                            skos:prefLabel "Electricity Indirect GHG Emission Indicator"@en .


###  http://www.fortiss.org/diprolea/ontosustain/rso#Emission
rso:Emission rdf:type owl:Class ;
             rdfs:subClassOf rso:Variable ;
             rdfs:comment "A variable that quantifies emissions."@en ;
             rdfs:label "Emission"@en ;
             skos:prefLabel "Emission"@en .


###  http://www.fortiss.org/diprolea/ontosustain/rso#EmissionIndicator
rso:EmissionIndicator rdf:type owl:Class ;
                      owl:equivalentClass [ owl:intersectionOf ( rso:Indicator
                                                                 [ rdf:type owl:Restriction ;
                                                                   owl:onProperty rso:hasMeasurementVariable ;
                                                                   owl:someValuesFrom rso:Emission
                                                                 ]
                                                               ) ;
                                            rdf:type owl:Class
                                          ] ;
                      rdfs:comment "Indicators measure the emission topic."@en ;
                      rdfs:label "Emission Indicator"@en ;
                      skos:prefLabel "Emission Indicator"@en .


###  http://www.fortiss.org/diprolea/ontosustain/rso#EnergyIndicator
rso:EnergyIndicator rdf:type owl:Class ;
                    owl:equivalentClass [ owl:intersectionOf ( rso:Indicator
                                                               [ rdf:type owl:Restriction ;
                                                                 owl:onProperty rso:hasMeasurementVariable ;
                                                                 owl:someValuesFrom rso:EnergyVariable
                                                               ]
                                                             ) ;
                                          rdf:type owl:Class
                                        ] ;
                    rdfs:comment "Indicators that measure the energy topic."@en ;
                    rdfs:label "Energy Indicator"@en ;
                    skos:prefLabel "Energy Indicator"@en .


###  http://www.fortiss.org/diprolea/ontosustain/rso#EnergyVariable
rso:EnergyVariable rdf:type owl:Class ;
                   rdfs:subClassOf rso:Variable ;
                   rdfs:comment "A variable that quantifies energy metrics."@en ;
                   rdfs:label "Energy"@en ;
                   skos:prefLabel "Energy"@en .


###  http://www.fortiss.org/diprolea/ontosustain/rso#EnvironmentalIndicator
rso:EnvironmentalIndicator rdf:type owl:Class ;
                           owl:equivalentClass [ owl:intersectionOf ( rso:Indicator
                                                                      [ rdf:type owl:Restriction ;
                                                                        owl:onProperty rso:measuresDimension ;
                                                                        owl:hasValue rso:Environment
                                                                      ]
                                                                    ) ;
                                                 rdf:type owl:Class
                                               ] ;
                           rdfs:comment "Indicators that measure the environmen dimension of sustainability."@en ;
                           rdfs:label "Environmental Indicator"@en ;
                           skos:prefLabel "Environmental Indicator"@en .


###  http://www.fortiss.org/diprolea/ontosustain/rso#GHGEmission
rso:GHGEmission rdf:type owl:Class ;
                rdfs:subClassOf rso:Emission ;
                rdfs:comment "Gas that contributes to the greenhouse effect by absorbing infrared radiation."@en ;
                rdfs:isDefinedBy "https://www.globalreporting.org/publications/documents/english/gri-305-emissions-2016/" ;
                rdfs:label "GHG Emission"@en ;
                skos:prefLabel "GHG Emission"@en .


###  http://www.fortiss.org/diprolea/ontosustain/rso#GHGEmissionIndicator
rso:GHGEmissionIndicator rdf:type owl:Class ;
                         owl:equivalentClass [ owl:intersectionOf ( rso:EmissionIndicator
                                                                    [ rdf:type owl:Restriction ;
                                                                      owl:onProperty rso:hasMeasurementVariable ;
                                                                      owl:someValuesFrom rso:GHGEmission
                                                                    ]
                                                                  ) ;
                                               rdf:type owl:Class
                                             ] ;
                         rdfs:comment "Indicator that measures the Green House Gas emissions subtopic."@en ;
                         rdfs:label "GHG Emission Indicator"@en ;
                         skos:prefLabel "GHG Emission Indicator" .


###  http://www.fortiss.org/diprolea/ontosustain/rso#GRIDisclosure
rso:GRIDisclosure rdf:type owl:Class ;
                  rdfs:subClassOf rso:Disclosure ;
                  rdfs:comment """The GRI Standards contain disclosures that allow an organization to report information about its impacts consistently and
credibly."""@en ;
                  rdfs:isDefinedBy "https://www.globalreporting.org/pdf.ashx?id=12334"^^xsd:anyURI ;
                  rdfs:label "GRI Disclosure"@en ;
                  skos:prefLabel "GRI Disclosure"@en .


###  http://www.fortiss.org/diprolea/ontosustain/rso#GRIEnvironmentTopic
rso:GRIEnvironmentTopic rdf:type owl:Class ;
                        rdfs:subClassOf rso:GRITopic ;
                        rdfs:comment "GRI topics derived from the GRI standards describing the environmental dimension."@en ;
                        rdfs:label "GRI Environment Topic"@en ;
                        skos:prefLabel "GRI Environment Topic"@en .


###  http://www.fortiss.org/diprolea/ontosustain/rso#GRIGovernanceTopic
rso:GRIGovernanceTopic rdf:type owl:Class ;
                       rdfs:subClassOf rso:GRITopic ;
                       rdfs:comment "GRI topics derived from the GRI standards describing the governance dimension."@en ;
                       rdfs:label "GRI Governance Topic"@en ;
                       skos:prefLabel "GRI Governance Topic"@en .


###  http://www.fortiss.org/diprolea/ontosustain/rso#GRIIndicator
rso:GRIIndicator rdf:type owl:Class ;
                 rdfs:subClassOf rso:Indicator ;
                 rdfs:comment "Indicators derived from the GRI standards."@en ;
                 rdfs:label "GRI Indicator"@en ;
                 skos:prefLabel "GRI Indicator"@en .


###  http://www.fortiss.org/diprolea/ontosustain/rso#GRISocialTopic
rso:GRISocialTopic rdf:type owl:Class ;
                   rdfs:subClassOf rso:GRITopic ;
                   rdfs:comment "GRI topics derived from the GRI standards describing the social dimension."@en ;
                   rdfs:label "GRI Social Topic"@en ;
                   skos:prefLabel "GRI Social Topic"@en .


###  http://www.fortiss.org/diprolea/ontosustain/rso#GRIStandard
rso:GRIStandard rdf:type owl:Class ;
                rdfs:subClassOf rso:Standard ;
                rdfs:comment "A GRI standard is a piece of the GRI Sustainability Reporting Standards (GRI Standards). For example, GRI 301: Materials 2016."@en ;
                rdfs:label "GRI Standard"@en ;
                skos:prefLabel "GRI Standard"@en .


###  http://www.fortiss.org/diprolea/ontosustain/rso#GRITopic
rso:GRITopic rdf:type owl:Class ;
             rdfs:subClassOf rso:Topic ;
             rdfs:comment "GRI topics derived from the GRI standards."@en ;
             rdfs:label "GRI Topic"@en ;
             skos:prefLabel "GRI Topic"@en .


###  http://www.fortiss.org/diprolea/ontosustain/rso#GRITopicStandard
rso:GRITopicStandard rdf:type owl:Class ;
                     rdfs:subClassOf rso:GRIStandard ;
                     owl:disjointWith rso:GRIUniversalStandard ;
                     rdfs:comment "The Topic Standards contain disclosures that the organization uses to report information about its impacts in relation to particular topics. The organization uses the Topic Standards according to the list of material topics it has determined using GRI 3."@en ;
                     rdfs:label "GRI Topic Standard"@en ;
                     skos:prefLabel "GRI Topic Standard"@en .


###  http://www.fortiss.org/diprolea/ontosustain/rso#GRIUniversalStandard
rso:GRIUniversalStandard rdf:type owl:Class ;
                         rdfs:subClassOf rso:GRIStandard ;
                         rdfs:comment """The Universal Standards defined in GRI standards are: GRI 1, GRI 2 and GRI 3
GRI 1: Foundation 2021 specifies the requirements that the organization must comply with to report in accordance with the GRI Standards. The organization begins using the GRI Standards by consulting GRI 1.
GRI 2: General Disclosures 2021 contains disclosures that the organization uses to provide information about its reporting practices and other organizational details, such as its activities, governance, and policies.
GRI 3: Material Topics 2021 provides guidance on how to determine material topics. It also contains disclosures that the organization uses to report information about its process of determining material topics, its list of material topics, and how it manages each topic."""@en ;
                         rdfs:label "GRI Universal Standard"@en ;
                         skos:prefLabel "GRI Universal Standard"@en .


###  http://www.fortiss.org/diprolea/ontosustain/rso#HAP
rso:HAP rdf:type owl:Class ;
        rdfs:subClassOf rso:OtherAirEmission ;
        rdfs:comment "Variables (measurement objects) regarding HAP."@en ;
        rdfs:isDefinedBy "https://www.globalreporting.org/publications/documents/english/gri-305-emissions-2016/" ;
        rdfs:label "Hazardous air pollutants (HAP)"@en ;
        skos:prefLabel "Hazardous air pollutants (HAP)"@en .


###  http://www.fortiss.org/diprolea/ontosustain/rso#HAPIndicator
rso:HAPIndicator rdf:type owl:Class ;
                 owl:equivalentClass [ owl:intersectionOf ( rso:OtherEmissionIndicator
                                                            [ rdf:type owl:Restriction ;
                                                              owl:onProperty rso:hasMeasurementVariable ;
                                                              owl:someValuesFrom rso:HAP
                                                            ]
                                                          ) ;
                                       rdf:type owl:Class
                                     ] ;
                 rdfs:comment "Indicator that measures Hazardous air pollutants (HAP) subtopic."@en ;
                 rdfs:label "Hazardous air pollutants (HAP) Indicator"@en ;
                 skos:prefLabel "Hazardous air pollutants (HAP) Indicator"@en .


###  http://www.fortiss.org/diprolea/ontosustain/rso#HazardousWasteDFDIndicator
rso:HazardousWasteDFDIndicator rdf:type owl:Class ;
                               owl:equivalentClass [ owl:intersectionOf ( rso:WasteDFDIndicator
                                                                          [ rdf:type owl:Restriction ;
                                                                            owl:onProperty rso:hasMeasurementVariable ;
                                                                            owl:someValuesFrom rso:HazardousWasteDivertedFromDisposal
                                                                          ]
                                                                        ) ;
                                                     rdf:type owl:Class
                                                   ] ;
                               rdfs:comment "Indicator that measures the hazardous waste diverted from disposal subtopic."@en ;
                               rdfs:label "Hazardous Diverted From Disposal Waste Inidicator"@en ;
                               skos:prefLabel "Hazardous Diverted From Disposal Waste Inidicator"@en .


###  http://www.fortiss.org/diprolea/ontosustain/rso#HazardousWasteDFDbyOtherRecoveryOptionsIndicator
rso:HazardousWasteDFDbyOtherRecoveryOptionsIndicator rdf:type owl:Class ;
                                                     owl:equivalentClass [ owl:intersectionOf ( rso:HazardousWasteDFDIndicator
                                                                                                [ rdf:type owl:Restriction ;
                                                                                                  owl:onProperty rso:hasMeasurementVariable ;
                                                                                                  owl:someValuesFrom rso:HazardousWasteWasteDFDbyOtherRecoveryOptions
                                                                                                ]
                                                                                              ) ;
                                                                           rdf:type owl:Class
                                                                         ] ;
                                                     rdfs:comment "Indicator that measures the hazardous waste diverted from disposal by other recovery options subtopic."@en ;
                                                     rdfs:label "Hazardous Diverted From Disposal by Other Recovery Options Waste Indicator"@en ;
                                                     skos:prefLabel "Hazardous Diverted From Disposal by Other Recovery Options Waste Indicator"@en .


###  http://www.fortiss.org/diprolea/ontosustain/rso#HazardousWasteDFDbyPreparationForReuseIndicator
rso:HazardousWasteDFDbyPreparationForReuseIndicator rdf:type owl:Class ;
                                                    owl:equivalentClass [ owl:intersectionOf ( rso:HazardousWasteDFDIndicator
                                                                                               [ rdf:type owl:Restriction ;
                                                                                                 owl:onProperty rso:hasMeasurementVariable ;
                                                                                                 owl:someValuesFrom rso:HazardousWasteWasteDFDbyPreparationForReuse
                                                                                               ]
                                                                                             ) ;
                                                                          rdf:type owl:Class
                                                                        ] ;
                                                    rdfs:comment "Indicator that measures the hazardous waste diverted from disposal by preperation for reuse subtopic."@en ;
                                                    rdfs:label "Hazardous Diverted From Disposal by Preparation For Reuse Waste Indicator"@en ;
                                                    skos:prefLabel "Hazardous Diverted From Disposal by Preparation For Reuse Waste Indicator"@en .


###  http://www.fortiss.org/diprolea/ontosustain/rso#HazardousWasteDFDbyRecyclingIndicator
rso:HazardousWasteDFDbyRecyclingIndicator rdf:type owl:Class ;
                                          owl:equivalentClass [ owl:intersectionOf ( rso:HazardousWasteDFDIndicator
                                                                                     [ rdf:type owl:Restriction ;
                                                                                       owl:onProperty rso:hasMeasurementVariable ;
                                                                                       owl:someValuesFrom rso:HazardousWasteWasteDFDbyRecycling
                                                                                     ]
                                                                                   ) ;
                                                                rdf:type owl:Class
                                                              ] ;
                                          rdfs:comment "Indicator that measures the hazardous waste diverted from disposal by recycling subtopic."@en ;
                                          rdfs:label "Hazardous Diverted From Disposal by Recycling Waste Indicator"@en ;
                                          skos:prefLabel "Hazardous Diverted From Disposal by Recycling Waste Indicator"@en .


###  http://www.fortiss.org/diprolea/ontosustain/rso#HazardousWasteDTDIndicator
rso:HazardousWasteDTDIndicator rdf:type owl:Class ;
                               owl:equivalentClass [ owl:intersectionOf ( rso:WasteDTDIndicator
                                                                          [ rdf:type owl:Restriction ;
                                                                            owl:onProperty rso:hasMeasurementVariable ;
                                                                            owl:someValuesFrom rso:HazardousWasteDirectedToDisposal
                                                                          ]
                                                                        ) ;
                                                     rdf:type owl:Class
                                                   ] ;
                               rdfs:comment "Indicator that measures the hazardous waste directed to disposal subtopic."@en ;
                               rdfs:label "Hazardous Directed To Disposal Waste Inidicator"@en ;
                               skos:prefLabel "Hazardous Directed To Disposal Waste Inidicator"@en .


###  http://www.fortiss.org/diprolea/ontosustain/rso#HazardousWasteDTDbyIncinerationIndicator
rso:HazardousWasteDTDbyIncinerationIndicator rdf:type owl:Class ;
                                             owl:equivalentClass [ owl:intersectionOf ( rso:HazardousWasteDTDIndicator
                                                                                        [ rdf:type owl:Restriction ;
                                                                                          owl:onProperty rso:hasMeasurementVariable ;
                                                                                          owl:someValuesFrom rso:HazardousWasteWasteDTDbyIncineration
                                                                                        ]
                                                                                      ) ;
                                                                   rdf:type owl:Class
                                                                 ] ;
                                             rdfs:comment "Indicator that measures the hazardous waste directed to disposal by incineration subtopic."@en ;
                                             rdfs:label "Hazardous Directed To Disposal by Incineration Waste Inidicator"@en ;
                                             skos:prefLabel "Hazardous Directed To Disposal by Incineration Waste Inidicator"@en .


###  http://www.fortiss.org/diprolea/ontosustain/rso#HazardousWasteDTDbyIncinerationWithEnergyRecoveryIndicator
rso:HazardousWasteDTDbyIncinerationWithEnergyRecoveryIndicator rdf:type owl:Class ;
                                                               owl:equivalentClass [ owl:intersectionOf ( rso:HazardousWasteDTDbyIncinerationIndicator
                                                                                                          [ rdf:type owl:Restriction ;
                                                                                                            owl:onProperty rso:hasMeasurementVariable ;
                                                                                                            owl:someValuesFrom rso:HazardousWasteWasteDTDbyIncinerationWithEnergyRecovery
                                                                                                          ]
                                                                                                        ) ;
                                                                                     rdf:type owl:Class
                                                                                   ] ;
                                                               rdfs:comment "Indicator that measures the hazardous waste directed to disposal by incineration with energy recovery subtopic."@en ;
                                                               rdfs:label "Hazardous Directed To Disposal by Incineration With Energy Recovery Waste Indicator"@en ;
                                                               skos:prefLabel "Hazardous Directed To Disposal by Incineration With Energy Recovery Waste Indicator"@en .


###  http://www.fortiss.org/diprolea/ontosustain/rso#HazardousWasteDTDbyIncinerationWithoutEnergyRecoveryIndicator
rso:HazardousWasteDTDbyIncinerationWithoutEnergyRecoveryIndicator rdf:type owl:Class ;
                                                                  owl:equivalentClass [ owl:intersectionOf ( rso:HazardousWasteDTDbyIncinerationIndicator
                                                                                                             [ rdf:type owl:Restriction ;
                                                                                                               owl:onProperty rso:hasMeasurementVariable ;
                                                                                                               owl:someValuesFrom rso:HazardousWasteWasteDTDbyIncinerationWithoutEnergyRecovery
                                                                                                             ]
                                                                                                           ) ;
                                                                                        rdf:type owl:Class
                                                                                      ] ;
                                                                  rdfs:comment "Indicator that measures the hazardous waste directed to disposal by incineration without energy recovery subtopic."@en ;
                                                                  rdfs:label "Hazardous Directed To Disposal by Incineration Without Energy Recovery Waste Indicator"@en ;
                                                                  skos:prefLabel "Hazardous Directed To Disposal by Incineration Without Energy Recovery Waste Indicator"@en .


###  http://www.fortiss.org/diprolea/ontosustain/rso#HazardousWasteDTDbyLandfillingIndicator
rso:HazardousWasteDTDbyLandfillingIndicator rdf:type owl:Class ;
                                            owl:equivalentClass [ owl:intersectionOf ( rso:HazardousWasteDTDIndicator
                                                                                       [ rdf:type owl:Restriction ;
                                                                                         owl:onProperty rso:hasMeasurementVariable ;
                                                                                         owl:someValuesFrom rso:HazardousWasteWasteDTDbyLandfilling
                                                                                       ]
                                                                                     ) ;
                                                                  rdf:type owl:Class
                                                                ] ;
                                            rdfs:comment "Indicator that measures the hazardous waste directed to disposal by landfilling subtopic."@en ;
                                            rdfs:label "Hazardous Directed To Disposal by Landfilling Waste Inidicator"@en ;
                                            skos:prefLabel "Hazardous Directed To Disposal by Landfilling Waste Inidicator"@en .


###  http://www.fortiss.org/diprolea/ontosustain/rso#HazardousWasteDTDbyOtherDisposalOperationsIndicator
rso:HazardousWasteDTDbyOtherDisposalOperationsIndicator rdf:type owl:Class ;
                                                        owl:equivalentClass [ owl:intersectionOf ( rso:HazardousWasteDTDIndicator
                                                                                                   [ rdf:type owl:Restriction ;
                                                                                                     owl:onProperty rso:hasMeasurementVariable ;
                                                                                                     owl:someValuesFrom rso:HazardousWasteWasteDTDbyOtherDisposalOperations
                                                                                                   ]
                                                                                                 ) ;
                                                                              rdf:type owl:Class
                                                                            ] ;
                                                        rdfs:comment "Indicator that measures the hazardous waste directed to disposal by other disposal operations subtopic."@en ;
                                                        rdfs:label "Hazardous Directed To Disposal by Other Disposal Operations Waste Inidicator"@en ;
                                                        skos:prefLabel "Hazardous Directed To Disposal by Other Disposal Operations Waste Inidicator"@en .


###  http://www.fortiss.org/diprolea/ontosustain/rso#HazardousWasteDirectedToDisposal
rso:HazardousWasteDirectedToDisposal rdf:type owl:Class ;
                                     rdfs:subClassOf rso:WasteDirectedToDisposal ;
                                     owl:disjointWith rso:NonHazardousWasteDirectedToDisposal ;
                                     rdfs:comment "Variables (measurement objects) regarding hazaardous waste directed to disposal."@en ;
                                     rdfs:label "Hazardous Waste Directed To Disposal"@en ;
                                     skos:prefLabel "Hazardous Waste Directed To Disposal"@en .


###  http://www.fortiss.org/diprolea/ontosustain/rso#HazardousWasteDivertedFromDisposal
rso:HazardousWasteDivertedFromDisposal rdf:type owl:Class ;
                                       rdfs:subClassOf rso:WasteDivertedFromDisposal ;
                                       owl:disjointWith rso:NonHazardousWasteDivertedFromDisposal ;
                                       rdfs:comment "Variables (measurement objects) regarding hazardous waste diverted from disposal."@en ;
                                       rdfs:label "Hazardous Waste Diverted From Disposal"@en ;
                                       skos:prefLabel "Hazardous Waste Diverted From Disposal"@en .


###  http://www.fortiss.org/diprolea/ontosustain/rso#HazardousWasteWasteDFDbyOtherRecoveryOptions
rso:HazardousWasteWasteDFDbyOtherRecoveryOptions rdf:type owl:Class ;
                                                 rdfs:subClassOf rso:HazardousWasteDivertedFromDisposal ;
                                                 rdfs:comment "Variables (measurement objects) regarding hazardous waste diverted from disposal by other recovery options."@en ;
                                                 rdfs:label "Hazardous Waste Diverted From Disposal by Other Recovery Options"@en ;
                                                 skos:prefLabel "Hazardous Waste Diverted From Disposal by Other Recovery Options"@en .


###  http://www.fortiss.org/diprolea/ontosustain/rso#HazardousWasteWasteDFDbyPreparationForReuse
rso:HazardousWasteWasteDFDbyPreparationForReuse rdf:type owl:Class ;
                                                rdfs:subClassOf rso:HazardousWasteDivertedFromDisposal ;
                                                rdfs:comment "Variables (measurement objects) regarding hazardous waste diverted from disposal by preparation for reuse."@en ;
                                                rdfs:label "Hazardous Waste Diverted From Disposal by Preparation For Reuse"@en ;
                                                skos:prefLabel "Hazardous Waste Diverted From Disposal by Preparation For Reuse"@en .


###  http://www.fortiss.org/diprolea/ontosustain/rso#HazardousWasteWasteDFDbyRecycling
rso:HazardousWasteWasteDFDbyRecycling rdf:type owl:Class ;
                                      rdfs:subClassOf rso:HazardousWasteDivertedFromDisposal ;
                                      rdfs:comment "Variables (measurement objects) regarding hazardous waste diverted from disposal by recycling, in which reprocessing of products or components of products that have become waste, to make new materials."@en ;
                                      rdfs:label "Hazardous Waste Diverted From Disposal by Recycling"@en ;
                                      skos:prefLabel "Hazardous Waste Diverted From Disposal by Recycling"@en .


###  http://www.fortiss.org/diprolea/ontosustain/rso#HazardousWasteWasteDTDbyIncineration
rso:HazardousWasteWasteDTDbyIncineration rdf:type owl:Class ;
                                         rdfs:subClassOf rso:HazardousWasteDirectedToDisposal ;
                                         rdfs:comment "Variables (measurement objects) regarding hazaardous waste directed to disposal by incineration, in which controlled burning of waste at high temperatures."@en ;
                                         rdfs:label "Hazardous Waste Directed To Disposal by Incineration"@en ;
                                         skos:prefLabel "Hazardous Waste Directed To Disposal by Incineration"@en .


###  http://www.fortiss.org/diprolea/ontosustain/rso#HazardousWasteWasteDTDbyIncinerationWithEnergyRecovery
rso:HazardousWasteWasteDTDbyIncinerationWithEnergyRecovery rdf:type owl:Class ;
                                                           rdfs:subClassOf rso:HazardousWasteWasteDTDbyIncineration ;
                                                           rdfs:comment "Variables (measurement objects) regarding hazaardous waste directed to disposal by incineration with energy recovery."@en ;
                                                           rdfs:label "Hazardous Waste Directed To Disposal by Incineration With Energy Recovery"@en ;
                                                           skos:prefLabel "Hazardous Waste Directed To Disposal by Incineration With Energy Recovery"@en .


###  http://www.fortiss.org/diprolea/ontosustain/rso#HazardousWasteWasteDTDbyIncinerationWithoutEnergyRecovery
rso:HazardousWasteWasteDTDbyIncinerationWithoutEnergyRecovery rdf:type owl:Class ;
                                                              rdfs:subClassOf rso:HazardousWasteWasteDTDbyIncineration ;
                                                              rdfs:comment "Variables (measurement objects) regarding hazaardous waste directed to disposal by incineration without energy recovery."@en ;
                                                              rdfs:label "Hazardous Waste Directed To Disposal by Incineration Without Energy Recovery"@en ;
                                                              skos:prefLabel "Hazardous Waste Directed To Disposal by Incineration Without Energy Recovery"@en .


###  http://www.fortiss.org/diprolea/ontosustain/rso#HazardousWasteWasteDTDbyLandfilling
rso:HazardousWasteWasteDTDbyLandfilling rdf:type owl:Class ;
                                        rdfs:subClassOf rso:HazardousWasteDirectedToDisposal ;
                                        rdfs:comment "Variables (measurement objects) regarding hazaardous waste directed to disposal by landfilling, in which final depositing of solid waste at, below, or above ground level at engineered disposal sites."@en ;
                                        rdfs:label "Hazardous Waste Directed To Disposal by Landfilling"@en ;
                                        skos:prefLabel "Hazardous Waste Directed To Disposal by Landfilling"@en .


###  http://www.fortiss.org/diprolea/ontosustain/rso#HazardousWasteWasteDTDbyOtherDisposalOperations
rso:HazardousWasteWasteDTDbyOtherDisposalOperations rdf:type owl:Class ;
                                                    rdfs:subClassOf rso:HazardousWasteDirectedToDisposal ;
                                                    rdfs:comment "Variables (measurement objects) regarding hazaardous waste directed to disposal by other disposal operations."@en ;
                                                    rdfs:label "Hazardous Waste Directed To Disposal by Other Disposal Operations"@en ;
                                                    skos:prefLabel "Hazardous Waste Directed To Disposal by Other Disposal Operations"@en .


###  http://www.fortiss.org/diprolea/ontosustain/rso#Indicator
rso:Indicator rdf:type owl:Class ;
              rdfs:comment "A single measure from which conclusions on the phenomenon of interest can be inferred."@en ;
              rdfs:label "Sustainability Indicator"@en ;
              skos:prefLabel "Sustainability Indicator"@en .


###  http://www.fortiss.org/diprolea/ontosustain/rso#IndirectGHGEmission
rso:IndirectGHGEmission rdf:type owl:Class ;
                        rdfs:subClassOf rso:GHGEmission ;
                        rdfs:comment "Scope 2 and Scope 3 emissions."@en ;
                        rdfs:isDefinedBy "https://www.globalreporting.org/publications/documents/english/gri-305-emissions-2016/" ;
                        rdfs:label "Indirect GHG Emission"@en ;
                        skos:prefLabel "Indirect GHG Emission"@en .


###  http://www.fortiss.org/diprolea/ontosustain/rso#IndirectGHGEmissionIndicator
rso:IndirectGHGEmissionIndicator rdf:type owl:Class ;
                                 owl:equivalentClass [ owl:intersectionOf ( rso:GHGEmissionIndicator
                                                                            [ rdf:type owl:Restriction ;
                                                                              owl:onProperty rso:hasMeasurementVariable ;
                                                                              owl:someValuesFrom rso:IndirectGHGEmission
                                                                            ]
                                                                          ) ;
                                                       rdf:type owl:Class
                                                     ] ;
                                 rdfs:comment "Indicator that measures the indirect GHG emission subtopic."@en ;
                                 rdfs:label "Indirect GHG Emission Indicator" ;
                                 skos:prefLabel "Indirect GHG Emission Indicator" .


###  http://www.fortiss.org/diprolea/ontosustain/rso#IntensityIndicator
rso:IntensityIndicator rdf:type owl:Class ;
                       rdfs:subClassOf rso:WeightedIndicator ;
                       rdfs:comment "An intensity indicator has different quantity kinds and units on numerator and denominator." ;
                       rdfs:label "Intensity Indicator"@en ;
                       skos:prefLabel "Intensity Indicator"@en .


###  http://www.fortiss.org/diprolea/ontosustain/rso#Material
rso:Material rdf:type owl:Class ;
             rdfs:subClassOf rso:Variable ;
             rdfs:comment "A variable that quantifies material usage."@en ;
             rdfs:label "Material"@en ;
             skos:prefLabel "Material"@en .


###  http://www.fortiss.org/diprolea/ontosustain/rso#MaterialIndicator
rso:MaterialIndicator rdf:type owl:Class ;
                      owl:equivalentClass [ owl:intersectionOf ( rso:Indicator
                                                                 [ rdf:type owl:Restriction ;
                                                                   owl:onProperty rso:hasMeasurementVariable ;
                                                                   owl:someValuesFrom rso:Material
                                                                 ]
                                                               ) ;
                                            rdf:type owl:Class
                                          ] ;
                      rdfs:comment "Indicators measure the material topic."@en ;
                      rdfs:label "Material Indicator"@en ;
                      skos:prefLabel "Material Indicator"@en .


###  http://www.fortiss.org/diprolea/ontosustain/rso#NOx
rso:NOx rdf:type owl:Class ;
        rdfs:subClassOf rso:OtherAirEmission ;
        rdfs:comment "Variables (measurement objects) regarding NOx."@en ;
        rdfs:isDefinedBy "https://www.globalreporting.org/publications/documents/english/gri-305-emissions-2016/" ;
        rdfs:label "NOx"@en ;
        skos:prefLabel "NOx"@en .


###  http://www.fortiss.org/diprolea/ontosustain/rso#NOxIndicator
rso:NOxIndicator rdf:type owl:Class ;
                 owl:equivalentClass [ owl:intersectionOf ( rso:OtherEmissionIndicator
                                                            [ rdf:type owl:Restriction ;
                                                              owl:onProperty rso:hasMeasurementVariable ;
                                                              owl:someValuesFrom rso:NOx
                                                            ]
                                                          ) ;
                                       rdf:type owl:Class
                                     ] ;
                 rdfs:comment "Indicator that measures NOx subtopic."@en ;
                 rdfs:label "NOx Emission Indicator"@en ;
                 skos:prefLabel "NOx Emission Indicator"@en .


###  http://www.fortiss.org/diprolea/ontosustain/rso#NonHazardousWasteDFDIndicator
rso:NonHazardousWasteDFDIndicator rdf:type owl:Class ;
                                  owl:equivalentClass [ owl:intersectionOf ( rso:WasteDFDIndicator
                                                                             [ rdf:type owl:Restriction ;
                                                                               owl:onProperty rso:hasMeasurementVariable ;
                                                                               owl:someValuesFrom rso:NonHazardousWasteDivertedFromDisposal
                                                                             ]
                                                                           ) ;
                                                        rdf:type owl:Class
                                                      ] ;
                                  rdfs:comment "Indicator that measures the non-hazardous waste diverted from disposal subtopic."@en ;
                                  rdfs:label "Non-Hazardous Diverted From Disposal Waste Inidicator"@en ;
                                  skos:prefLabel "Non-Hazardous Diverted From Disposal Waste Inidicator"@en .


###  http://www.fortiss.org/diprolea/ontosustain/rso#NonHazardousWasteDFDbyOtherRecoveryOptionsIndicator
rso:NonHazardousWasteDFDbyOtherRecoveryOptionsIndicator rdf:type owl:Class ;
                                                        owl:equivalentClass [ owl:intersectionOf ( rso:NonHazardousWasteDFDIndicator
                                                                                                   [ rdf:type owl:Restriction ;
                                                                                                     owl:onProperty rso:hasMeasurementVariable ;
                                                                                                     owl:someValuesFrom rso:NonHazardousWasteWasteDFDbyOtherRecoveryOptions
                                                                                                   ]
                                                                                                 ) ;
                                                                              rdf:type owl:Class
                                                                            ] ;
                                                        rdfs:comment "Indicator that measures the non-hazardous waste diverted from disposal by other recovery options subtopic."@en ;
                                                        rdfs:label "Non-Hazardous Diverted From Disposal by Other Recovery Options Waste Indicator"@en ;
                                                        skos:prefLabel "Non-Hazardous Diverted From Disposal by Other Recovery Options Waste Indicator"@en .


###  http://www.fortiss.org/diprolea/ontosustain/rso#NonHazardousWasteDFDbyPreparationForReuseIndicator
rso:NonHazardousWasteDFDbyPreparationForReuseIndicator rdf:type owl:Class ;
                                                       owl:equivalentClass [ owl:intersectionOf ( rso:NonHazardousWasteDFDIndicator
                                                                                                  [ rdf:type owl:Restriction ;
                                                                                                    owl:onProperty rso:hasMeasurementVariable ;
                                                                                                    owl:someValuesFrom rso:NonHazardousWasteWasteDFDbyPreparationForReuse
                                                                                                  ]
                                                                                                ) ;
                                                                             rdf:type owl:Class
                                                                           ] ;
                                                       rdfs:comment "Indicator that measures the non-hazardous waste diverted from disposal by preparation for reuse subtopic."@en ;
                                                       rdfs:label "Non-Hazardous Diverted From Disposal by Preparation For Reuse Waste Indicator"@en ;
                                                       skos:prefLabel "Non-Hazardous Diverted From Disposal by Preparation For Reuse Waste Indicator"@en .


###  http://www.fortiss.org/diprolea/ontosustain/rso#NonHazardousWasteDFDbyRecyclingIndicator
rso:NonHazardousWasteDFDbyRecyclingIndicator rdf:type owl:Class ;
                                             owl:equivalentClass [ owl:intersectionOf ( rso:NonHazardousWasteDFDIndicator
                                                                                        [ rdf:type owl:Restriction ;
                                                                                          owl:onProperty rso:hasMeasurementVariable ;
                                                                                          owl:someValuesFrom rso:NonHazardousWasteWasteDFDbyRecycling
                                                                                        ]
                                                                                      ) ;
                                                                   rdf:type owl:Class
                                                                 ] ;
                                             rdfs:comment "Indicator that measures the non-hazardous waste diverted from disposal by recycling subtopic."@en ;
                                             rdfs:label "Non-Hazardous Diverted From Disposal by Recycling Waste Indicator"@en ;
                                             skos:prefLabel "Non-Hazardous Diverted From Disposal by Recycling Waste Indicator"@en .


###  http://www.fortiss.org/diprolea/ontosustain/rso#NonHazardousWasteDTDIndicator
rso:NonHazardousWasteDTDIndicator rdf:type owl:Class ;
                                  owl:equivalentClass [ owl:intersectionOf ( rso:WasteDTDIndicator
                                                                             [ rdf:type owl:Restriction ;
                                                                               owl:onProperty rso:hasMeasurementVariable ;
                                                                               owl:someValuesFrom rso:NonHazardousWasteDirectedToDisposal
                                                                             ]
                                                                           ) ;
                                                        rdf:type owl:Class
                                                      ] ;
                                  rdfs:comment "Indicator that measures the non-hazardous waste directed to disposal subtopic."@en ;
                                  rdfs:label "Non-Hazardous Directed To Disposal Waste Inidicator"@en ;
                                  skos:prefLabel "Non-Hazardous Directed To Disposal Waste Inidicator"@en .


###  http://www.fortiss.org/diprolea/ontosustain/rso#NonHazardousWasteDTDbyIncinerationIndicator
rso:NonHazardousWasteDTDbyIncinerationIndicator rdf:type owl:Class ;
                                                owl:equivalentClass [ owl:intersectionOf ( rso:NonHazardousWasteDTDIndicator
                                                                                           [ rdf:type owl:Restriction ;
                                                                                             owl:onProperty rso:hasMeasurementVariable ;
                                                                                             owl:someValuesFrom rso:NonHazardousWasteWasteDTDbyIncineration
                                                                                           ]
                                                                                         ) ;
                                                                      rdf:type owl:Class
                                                                    ] ;
                                                rdfs:comment "Indicator that measures the non-hazardous waste directed to disposal by incineration subtopic."@en ;
                                                rdfs:label "Non-Hazardous Directed To Disposal by Incineration Waste Inidicator"@en ;
                                                skos:prefLabel "Non-Hazardous Directed To Disposal by Incineration Waste Inidicator"@en .


###  http://www.fortiss.org/diprolea/ontosustain/rso#NonHazardousWasteDTDbyIncinerationWithEnergyRecoveryIndicator
rso:NonHazardousWasteDTDbyIncinerationWithEnergyRecoveryIndicator rdf:type owl:Class ;
                                                                  owl:equivalentClass [ owl:intersectionOf ( rso:NonHazardousWasteDTDbyIncinerationIndicator
                                                                                                             [ rdf:type owl:Restriction ;
                                                                                                               owl:onProperty rso:hasMeasurementVariable ;
                                                                                                               owl:someValuesFrom rso:NonHazardousWasteWasteDTDbyIncinerationWithEnergyRecovery
                                                                                                             ]
                                                                                                           ) ;
                                                                                        rdf:type owl:Class
                                                                                      ] ;
                                                                  rdfs:comment "Indicator that measures the non-hazardous waste directed to disposal by incineration with energy recovery subtopic."@en ;
                                                                  rdfs:label "Non-Hazardous Directed To Disposal by Incineration With Energy Recovery Waste Indicator"@en ;
                                                                  skos:prefLabel "Non-Hazardous Directed To Disposal by Incineration With Energy Recovery Waste Indicator"@en .


###  http://www.fortiss.org/diprolea/ontosustain/rso#NonHazardousWasteDTDbyIncinerationWithoutEnergyRecoveryIndicator
rso:NonHazardousWasteDTDbyIncinerationWithoutEnergyRecoveryIndicator rdf:type owl:Class ;
                                                                     owl:equivalentClass [ owl:intersectionOf ( rso:NonHazardousWasteDTDbyIncinerationIndicator
                                                                                                                [ rdf:type owl:Restriction ;
                                                                                                                  owl:onProperty rso:hasMeasurementVariable ;
                                                                                                                  owl:someValuesFrom rso:NonHazardousWasteWasteDTDbyIncinerationWithoutEnergyRecovery
                                                                                                                ]
                                                                                                              ) ;
                                                                                           rdf:type owl:Class
                                                                                         ] ;
                                                                     rdfs:comment "Indicator that measures the non-hazardous waste directed to disposal by incineration without energy recovery subtopic."@en ;
                                                                     rdfs:label "Non-Hazardous Directed To Disposal by Incineration Without Energy Recovery Waste Indicator"@en ;
                                                                     skos:prefLabel "Non-Hazardous Directed To Disposal by Incineration Without Energy Recovery Waste Indicator"@en .


###  http://www.fortiss.org/diprolea/ontosustain/rso#NonHazardousWasteDTDbyLandfillingIndicator
rso:NonHazardousWasteDTDbyLandfillingIndicator rdf:type owl:Class ;
                                               owl:equivalentClass [ owl:intersectionOf ( rso:NonHazardousWasteDTDIndicator
                                                                                          [ rdf:type owl:Restriction ;
                                                                                            owl:onProperty rso:hasMeasurementVariable ;
                                                                                            owl:someValuesFrom rso:NonHazardousWasteWasteDTDbyLandfilling
                                                                                          ]
                                                                                        ) ;
                                                                     rdf:type owl:Class
                                                                   ] ;
                                               rdfs:comment "Indicator that measures the non-hazardous waste directed to disposal by landfilling subtopic."@en ;
                                               rdfs:label "Non-Hazardous Directed To Disposal by Landfilling Waste Inidicator"@en ;
                                               skos:prefLabel "Non-Hazardous Directed To Disposal by Landfilling Waste Inidicator"@en .


###  http://www.fortiss.org/diprolea/ontosustain/rso#NonHazardousWasteDTDbyOtherDisposalOperationsIndicator
rso:NonHazardousWasteDTDbyOtherDisposalOperationsIndicator rdf:type owl:Class ;
                                                           owl:equivalentClass [ owl:intersectionOf ( rso:NonHazardousWasteDTDIndicator
                                                                                                      [ rdf:type owl:Restriction ;
                                                                                                        owl:onProperty rso:hasMeasurementVariable ;
                                                                                                        owl:someValuesFrom rso:NonHazardousWasteWasteDTDbyOtherDisposalOperations
                                                                                                      ]
                                                                                                    ) ;
                                                                                 rdf:type owl:Class
                                                                               ] ;
                                                           rdfs:comment "Indicator that measures the non-hazardous waste directed to disposal by other disposal operations subtopic."@en ;
                                                           rdfs:label "Non-Hazardous Directed To Disposal by Other Disposal Operations Waste Inidicator"@en ;
                                                           skos:prefLabel "Non-Hazardous Directed To Disposal by Other Disposal Operations Waste Inidicator"@en .


###  http://www.fortiss.org/diprolea/ontosustain/rso#NonHazardousWasteDirectedToDisposal
rso:NonHazardousWasteDirectedToDisposal rdf:type owl:Class ;
                                        rdfs:subClassOf rso:WasteDirectedToDisposal ;
                                        rdfs:comment "Variables (measurement objects) regarding non-hazaardous waste directed to disposal."@en ;
                                        rdfs:label "Non-Hazardous Waste Directed To Disposal"@en ;
                                        skos:prefLabel "Non-Hazardous Waste Directed To Disposal"@en .


###  http://www.fortiss.org/diprolea/ontosustain/rso#NonHazardousWasteDivertedFromDisposal
rso:NonHazardousWasteDivertedFromDisposal rdf:type owl:Class ;
                                          rdfs:subClassOf rso:WasteDivertedFromDisposal ;
                                          rdfs:comment "Variables (measurement objects) regarding non-hazardous waste diverted from disposal."@en ;
                                          rdfs:label "Non-Hazardous Waste Diverted From Disposal"@en ;
                                          skos:prefLabel "Non-Hazardous Waste Diverted From Disposal"@en .


###  http://www.fortiss.org/diprolea/ontosustain/rso#NonHazardousWasteWasteDFDbyOtherRecoveryOptions
rso:NonHazardousWasteWasteDFDbyOtherRecoveryOptions rdf:type owl:Class ;
                                                    rdfs:subClassOf rso:NonHazardousWasteDivertedFromDisposal ;
                                                    rdfs:comment "Variables (measurement objects) regarding non-hazardous waste diverted from disposal by other recovery options."@en ;
                                                    rdfs:label "Non-Hazardous Waste Diverted From Disposal by Other Recovery Options"@en ;
                                                    skos:prefLabel "Non-Hazardous Waste Diverted From Disposal by Other Recovery Options"@en .


###  http://www.fortiss.org/diprolea/ontosustain/rso#NonHazardousWasteWasteDFDbyPreparationForReuse
rso:NonHazardousWasteWasteDFDbyPreparationForReuse rdf:type owl:Class ;
                                                   rdfs:subClassOf rso:NonHazardousWasteDivertedFromDisposal ;
                                                   rdfs:comment "Variables (measurement objects) regarding non-hazardous waste diverted from disposal by preparation for reuse."@en ;
                                                   rdfs:label "Non-Hazardous Waste Diverted From Disposal by Preparation For Reuse"@en ;
                                                   skos:prefLabel "Non-Hazardous Waste Diverted From Disposal by Preparation For Reuse"@en .


###  http://www.fortiss.org/diprolea/ontosustain/rso#NonHazardousWasteWasteDFDbyRecycling
rso:NonHazardousWasteWasteDFDbyRecycling rdf:type owl:Class ;
                                         rdfs:subClassOf rso:NonHazardousWasteDivertedFromDisposal ;
                                         rdfs:comment "Variables (measurement objects) regarding non-hazardous waste diverted from disposal by recycling, in which reprocessing of products or components of products that have become waste, to make new materials."@en ;
                                         rdfs:label "Non-Hazardous Waste Diverted From Disposal by Recycling"@en ;
                                         skos:prefLabel "Non-Hazardous Waste Diverted From Disposal by Recycling"@en .


###  http://www.fortiss.org/diprolea/ontosustain/rso#NonHazardousWasteWasteDTDbyIncineration
rso:NonHazardousWasteWasteDTDbyIncineration rdf:type owl:Class ;
                                            rdfs:subClassOf rso:NonHazardousWasteDirectedToDisposal ;
                                            rdfs:comment "Variables (measurement objects) regarding non-hazaardous waste directed to disposal by incineration, in which controlled burning of waste at high temperatures."@en ;
                                            rdfs:label "Non-Hazardous Waste Directed To Disposal by Incineration"@en ;
                                            skos:prefLabel "Non-Hazardous Waste Directed To Disposal by Incineration"@en .


###  http://www.fortiss.org/diprolea/ontosustain/rso#NonHazardousWasteWasteDTDbyIncinerationWithEnergyRecovery
rso:NonHazardousWasteWasteDTDbyIncinerationWithEnergyRecovery rdf:type owl:Class ;
                                                              rdfs:subClassOf rso:NonHazardousWasteWasteDTDbyIncineration ;
                                                              rdfs:comment "Variables (measurement objects) regarding non-hazaardous waste directed to disposal by incineration with energy recovery."@en ;
                                                              rdfs:label "Non-Hazardous Waste Directed To Disposal by Incineration With Energy Recovery"@en ;
                                                              skos:prefLabel "Non-Hazardous Waste Directed To Disposal by Incineration With Energy Recovery"@en .


###  http://www.fortiss.org/diprolea/ontosustain/rso#NonHazardousWasteWasteDTDbyIncinerationWithoutEnergyRecovery
rso:NonHazardousWasteWasteDTDbyIncinerationWithoutEnergyRecovery rdf:type owl:Class ;
                                                                 rdfs:subClassOf rso:NonHazardousWasteWasteDTDbyIncineration ;
                                                                 rdfs:comment "Variables (measurement objects) regarding non-hazaardous waste directed to disposal by incineration without energy recovery."@en ;
                                                                 rdfs:label "Non-Hazardous Waste Directed To Disposal by Incineration Without Energy Recovery"@en ;
                                                                 skos:prefLabel "Non-Hazardous Waste Directed To Disposal by Incineration Without Energy Recovery"@en .


###  http://www.fortiss.org/diprolea/ontosustain/rso#NonHazardousWasteWasteDTDbyLandfilling
rso:NonHazardousWasteWasteDTDbyLandfilling rdf:type owl:Class ;
                                           rdfs:subClassOf rso:NonHazardousWasteDirectedToDisposal ;
                                           rdfs:comment "Variables (measurement objects) regarding non-hazaardous waste directed to disposal by landfilling, in which final depositing of solid waste at, below, or above ground level at engineered disposal sites."@en ;
                                           rdfs:label "Non-Hazardous Waste Directed To Disposal by Landfilling"@en ;
                                           skos:prefLabel "Non-Hazardous Waste Directed To Disposal by Landfilling"@en .


###  http://www.fortiss.org/diprolea/ontosustain/rso#NonHazardousWasteWasteDTDbyOtherDisposalOperations
rso:NonHazardousWasteWasteDTDbyOtherDisposalOperations rdf:type owl:Class ;
                                                       rdfs:subClassOf rso:NonHazardousWasteDirectedToDisposal ;
                                                       rdfs:comment "Variables (measurement objects) regarding non-hazaardous waste directed to disposal by other disposal operations."@en ;
                                                       rdfs:label "Non-Hazardous Waste Directed To Disposal by Other Disposal Operations"@en ;
                                                       skos:prefLabel "Non-Hazardous Waste Directed To Disposal by Other Disposal Operations"@en .


###  http://www.fortiss.org/diprolea/ontosustain/rso#NonRecycledWaste
rso:NonRecycledWaste rdf:type owl:Class ;
                     rdfs:subClassOf rso:Waste ;
                     rdfs:comment "Variables (measurement objects) regarding non-recyled waste."@en ;
                     rdfs:label "Nonrecycled Waste"@en ;
                     skos:prefLabel "Nonrecycled Waste"@en .


###  http://www.fortiss.org/diprolea/ontosustain/rso#NonRecycledWasteIndicator
rso:NonRecycledWasteIndicator rdf:type owl:Class ;
                              owl:equivalentClass [ owl:intersectionOf ( rso:WasteIndicator
                                                                         [ rdf:type owl:Restriction ;
                                                                           owl:onProperty rso:hasMeasurementVariable ;
                                                                           owl:someValuesFrom rso:NonRecycledWaste
                                                                         ]
                                                                       ) ;
                                                    rdf:type owl:Class
                                                  ] ;
                              rdfs:comment "Indicator that measures the non-recycled waste subtopic."@en ;
                              rdfs:label "Non-Recycled Waste Indicator"@en ;
                              skos:prefLabel "Non-Recycled Waste Indicator"@en .


###  http://www.fortiss.org/diprolea/ontosustain/rso#NonRenewableMaterial
rso:NonRenewableMaterial rdf:type owl:Class ;
                         rdfs:subClassOf rso:Material ;
                         owl:disjointWith rso:RenewableMaterial ;
                         rdfs:comment "Resource that does not renew in short time periods."@en ;
                         rdfs:isDefinedBy "https://www.globalreporting.org/pdf.ashx?id=12456" ;
                         rdfs:label "Nonrenewable Material"@en ;
                         skos:prefLabel "Nonrenewable Material"@en .


###  http://www.fortiss.org/diprolea/ontosustain/rso#NonRenewableMaterialIndicator
rso:NonRenewableMaterialIndicator rdf:type owl:Class ;
                                  owl:equivalentClass [ owl:intersectionOf ( rso:MaterialIndicator
                                                                             [ rdf:type owl:Restriction ;
                                                                               owl:onProperty rso:hasMeasurementVariable ;
                                                                               owl:someValuesFrom rso:NonRenewableMaterial
                                                                             ]
                                                                           ) ;
                                                        rdf:type owl:Class
                                                      ] ;
                                  owl:disjointWith rso:RenewableMaterialIndicator ;
                                  rdfs:comment "Indicator that measures the non-renewable materials subtopic."@en ;
                                  rdfs:label "Non-Renewable Material Indicator"@en ;
                                  skos:prefLabel "Non-Renewable Material Indicator"@en .


###  http://www.fortiss.org/diprolea/ontosustain/rso#ODSEmission
rso:ODSEmission rdf:type owl:Class ;
                rdfs:subClassOf rso:Emission ;
                rdfs:comment """Substance with an ozone depletion potential (ODP) greater than 0 that can deplete the
stratospheric ozone layer."""@en ;
                rdfs:isDefinedBy "https://www.globalreporting.org/publications/documents/english/gri-305-emissions-2016/" ;
                rdfs:label "ODS Emission"@en ;
                skos:prefLabel "ODS Emission"@en .


###  http://www.fortiss.org/diprolea/ontosustain/rso#ODSEmissionIndicator
rso:ODSEmissionIndicator rdf:type owl:Class ;
                         owl:equivalentClass [ owl:intersectionOf ( rso:EmissionIndicator
                                                                    [ rdf:type owl:Restriction ;
                                                                      owl:onProperty rso:hasMeasurementVariable ;
                                                                      owl:someValuesFrom rso:ODSEmission
                                                                    ]
                                                                  ) ;
                                               rdf:type owl:Class
                                             ] ;
                         rdfs:comment "Indicator that measures the Ozone-Depleting Substances subtopic."@en ;
                         rdfs:label "ODS Emission Indicator" ;
                         skos:prefLabel "ODS Emission Indicator" .


###  http://www.fortiss.org/diprolea/ontosustain/rso#OtherAirEmission
rso:OtherAirEmission rdf:type owl:Class ;
                     rdfs:subClassOf rso:Emission ;
                     rdfs:comment "Nitrogen oxides (NOx), sulfur oxides (SOx), and other significant air emissions."@en ;
                     rdfs:isDefinedBy "https://www.globalreporting.org/publications/documents/english/gri-305-emissions-2016/" ;
                     rdfs:label "Other standard categories of air emissions identified in relevant regulations"@en ;
                     skos:prefLabel "Other standard categories of air emissions identified in relevant regulations"@en .


###  http://www.fortiss.org/diprolea/ontosustain/rso#OtherEmissionIndicator
rso:OtherEmissionIndicator rdf:type owl:Class ;
                           owl:equivalentClass [ owl:intersectionOf ( rso:EmissionIndicator
                                                                      [ rdf:type owl:Restriction ;
                                                                        owl:onProperty rso:hasMeasurementVariable ;
                                                                        owl:someValuesFrom rso:OtherAirEmission
                                                                      ]
                                                                    ) ;
                                                 rdf:type owl:Class
                                               ] ;
                           rdfs:comment "Indicator that measures other significant air emissions subtopic."@en ;
                           rdfs:label "Other Emission Indicator" ;
                           skos:prefLabel "Other Emission Indicator" .


###  http://www.fortiss.org/diprolea/ontosustain/rso#OtherIndirectGHGEmission
rso:OtherIndirectGHGEmission rdf:type owl:Class ;
                             rdfs:subClassOf rso:IndirectGHGEmission ;
                             rdfs:comment "Scope 3 GHG emissions, indirect greenhouse gas (GHG) emissions not included in energy indirect (Scope 2) GHG emissions that occur outside of the organization, including both upstream and downstream emissions."@en ;
                             rdfs:isDefinedBy "https://www.globalreporting.org/publications/documents/english/gri-305-emissions-2016/" ;
                             rdfs:label "Other indirect GHG emission"@en ;
                             skos:prefLabel "Other indirect GHG emission"@en .


###  http://www.fortiss.org/diprolea/ontosustain/rso#OtherIndirectGHGEmissionIndicator
rso:OtherIndirectGHGEmissionIndicator rdf:type owl:Class ;
                                      owl:equivalentClass [ owl:intersectionOf ( rso:IndirectGHGEmissionIndicator
                                                                                 [ rdf:type owl:Restriction ;
                                                                                   owl:onProperty rso:hasMeasurementVariable ;
                                                                                   owl:someValuesFrom rso:OtherIndirectGHGEmission
                                                                                 ]
                                                                               ) ;
                                                            rdf:type owl:Class
                                                          ] ;
                                      rdfs:comment "Indicator that measures other indirect GHG (scope 3) emission subtopic."@en ;
                                      rdfs:label "Other Indirect GHG Emission Indicator"@en ;
                                      skos:prefLabel "Other Indirect GHG Emission Indicator"@en .


###  http://www.fortiss.org/diprolea/ontosustain/rso#PM
rso:PM rdf:type owl:Class ;
       rdfs:subClassOf rso:OtherAirEmission ;
       rdfs:comment "Variables (measurement objects) regarding PM."@en ;
       rdfs:isDefinedBy "https://www.globalreporting.org/publications/documents/english/gri-305-emissions-2016/" ;
       rdfs:label "Particulate matter (PM)"@en ;
       skos:prefLabel "Particulate matter (PM)"@en .


###  http://www.fortiss.org/diprolea/ontosustain/rso#PMIndicator
rso:PMIndicator rdf:type owl:Class ;
                owl:equivalentClass [ owl:intersectionOf ( rso:OtherEmissionIndicator
                                                           [ rdf:type owl:Restriction ;
                                                             owl:onProperty rso:hasMeasurementVariable ;
                                                             owl:someValuesFrom rso:PM
                                                           ]
                                                         ) ;
                                      rdf:type owl:Class
                                    ] ;
                rdfs:comment "Indicator that measures Particulate matter (PM) subtopic."@en ;
                rdfs:label "Particulate matter (PM) Indicator"@en ;
                skos:prefLabel "Particulate matter (PM) Indicator"@en .


###  http://www.fortiss.org/diprolea/ontosustain/rso#POP
rso:POP rdf:type owl:Class ;
        rdfs:subClassOf rso:OtherAirEmission ;
        rdfs:comment "Variables (measurement objects) regarding POP."@en ;
        rdfs:isDefinedBy "https://www.globalreporting.org/publications/documents/english/gri-305-emissions-2016/" ;
        rdfs:label "Persistent organic pollutants (POP)"@en ;
        skos:prefLabel "Persistent organic pollutants (POP)"@en .


###  http://www.fortiss.org/diprolea/ontosustain/rso#POPIndicator
rso:POPIndicator rdf:type owl:Class ;
                 owl:equivalentClass [ owl:intersectionOf ( rso:OtherEmissionIndicator
                                                            [ rdf:type owl:Restriction ;
                                                              owl:onProperty rso:hasMeasurementVariable ;
                                                              owl:someValuesFrom rso:POP
                                                            ]
                                                          ) ;
                                       rdf:type owl:Class
                                     ] ;
                 rdfs:comment "Indicator that measures Persistent organic pollutants (POP) subtopic."@en ;
                 rdfs:label "Persistent organic pollutants (POP) Indicator"@en ;
                 skos:prefLabel "Persistent organic pollutants (POP) Indicator"@en .


###  http://www.fortiss.org/diprolea/ontosustain/rso#PercentageIndicator
rso:PercentageIndicator rdf:type owl:Class ;
                        rdfs:subClassOf rso:WeightedIndicator ;
                        rdfs:comment "A percentage indicator shares the same quantity kind on both numerator and denominator."@en ;
                        rdfs:label "Percentage Indicator"@en ;
                        skos:prefLabel "Percentage Indicator"@en .


###  http://www.fortiss.org/diprolea/ontosustain/rso#ProducedEnergy
rso:ProducedEnergy rdf:type owl:Class ;
                   rdfs:subClassOf rso:EnergyVariable ;
                   rdfs:comment "Variables (measurement objects) regarding organizational produced energy."@en ;
                   rdfs:label "Produced Energy"@en ;
                   skos:prefLabel "Produced Energy"@en .


###  http://www.fortiss.org/diprolea/ontosustain/rso#ProducedEnergyIndicator
rso:ProducedEnergyIndicator rdf:type owl:Class ;
                            owl:equivalentClass [ owl:intersectionOf ( rso:EnergyIndicator
                                                                       [ rdf:type owl:Restriction ;
                                                                         owl:onProperty rso:hasMeasurementVariable ;
                                                                         owl:someValuesFrom rso:ProducedEnergy
                                                                       ]
                                                                     ) ;
                                                  rdf:type owl:Class
                                                ] ;
                            rdfs:comment "Indicator that measures the produced energy subtopic."@en ;
                            rdfs:label "Produced Energy Indicator"@en ;
                            skos:prefLabel "Produced Energy Indicator"@en .


###  http://www.fortiss.org/diprolea/ontosustain/rso#ProducedNonRenewableEnergy
rso:ProducedNonRenewableEnergy rdf:type owl:Class ;
                               rdfs:subClassOf rso:ProducedEnergy ;
                               owl:disjointWith rso:ProducedRenewableEnergy ;
                               rdfs:comment "Variables (measurement objects) regarding organizational produced non-renewable energy."@en ;
                               rdfs:label "Produced Nonrenewable Energy"@en ;
                               skos:prefLabel "Produced Nonrenewable Energy"@en .


###  http://www.fortiss.org/diprolea/ontosustain/rso#ProducedNonRenewableEnergyIndicator
rso:ProducedNonRenewableEnergyIndicator rdf:type owl:Class ;
                                        owl:equivalentClass [ owl:intersectionOf ( rso:ProducedEnergyIndicator
                                                                                   [ rdf:type owl:Restriction ;
                                                                                     owl:onProperty rso:hasMeasurementVariable ;
                                                                                     owl:someValuesFrom rso:ProducedNonRenewableEnergy
                                                                                   ]
                                                                                 ) ;
                                                              rdf:type owl:Class
                                                            ] ;
                                        rdfs:comment "Indicator that measures the produced non-renewable energy subtopic."@en ;
                                        rdfs:label "Produced Non-Renewable Energy Indicator"@en ;
                                        skos:prefLabel "Produced Non-Renewable Energy Indicator"@en .


###  http://www.fortiss.org/diprolea/ontosustain/rso#ProducedRenewableEnergy
rso:ProducedRenewableEnergy rdf:type owl:Class ;
                            rdfs:subClassOf rso:ProducedEnergy ;
                            rdfs:comment "Variables (measurement objects) regarding organizational produced renewable energy."@en ;
                            rdfs:label "Produced Renewable Energy"@en ;
                            skos:prefLabel "Produced Renewable Energy"@en .


###  http://www.fortiss.org/diprolea/ontosustain/rso#ProducedRenewableEnergyIndicator
rso:ProducedRenewableEnergyIndicator rdf:type owl:Class ;
                                     owl:equivalentClass [ owl:intersectionOf ( rso:ProducedEnergyIndicator
                                                                                [ rdf:type owl:Restriction ;
                                                                                  owl:onProperty rso:hasMeasurementVariable ;
                                                                                  owl:someValuesFrom rso:ProducedRenewableEnergy
                                                                                ]
                                                                              ) ;
                                                           rdf:type owl:Class
                                                         ] ;
                                     rdfs:comment "Indicator that measures the produced renewable energy subtopic."@en ;
                                     rdfs:label "Produced Renewable Energy Indicator"@en ;
                                     skos:prefLabel "Produced Renewable Energy Indicator"@en .


###  http://www.fortiss.org/diprolea/ontosustain/rso#RenewableMaterial
rso:RenewableMaterial rdf:type owl:Class ;
                      rdfs:subClassOf rso:Material ;
                      rdfs:comment "Material that is derived from plentiful resources that are quickly replenished by ecological cycles or agricultural processes, so that the services provided by these and other linked resources are not endangered and remain available for the next generation."@en ;
                      rdfs:isDefinedBy "https://www.globalreporting.org/pdf.ashx?id=12456" ;
                      rdfs:label "Renewable Material"@en ;
                      skos:prefLabel "Renewable Material"@en .


###  http://www.fortiss.org/diprolea/ontosustain/rso#RenewableMaterialIndicator
rso:RenewableMaterialIndicator rdf:type owl:Class ;
                               owl:equivalentClass [ owl:intersectionOf ( rso:MaterialIndicator
                                                                          [ rdf:type owl:Restriction ;
                                                                            owl:onProperty rso:hasMeasurementVariable ;
                                                                            owl:someValuesFrom rso:RenewableMaterial
                                                                          ]
                                                                        ) ;
                                                     rdf:type owl:Class
                                                   ] ;
                               rdfs:comment "Indicator that measures the renewable materials subtopic."@en ;
                               rdfs:label "Renewable Material Indicator"@en ;
                               skos:prefLabel "Renewable Material Indicator"@en .


###  http://www.fortiss.org/diprolea/ontosustain/rso#Report
rso:Report rdf:type owl:Class ;
           rdfs:comment "Represents the annual sustainability report published by a certain organization and complies with certain standards."@en ;
           rdfs:label "Sustainability Report"@en ;
           skos:prefLabel "Sustainability Report"@en .


###  http://www.fortiss.org/diprolea/ontosustain/rso#ReportValue
rso:ReportValue rdf:type owl:Class ;
                rdfs:subClassOf rso:Value ;
                rdfs:comment "Provides a structure to represent a single report data. Each data contains a numerical value and a measurement unit and is linked to a specific indicator."@en ;
                rdfs:label "Sustaianbility Report Value"@en ;
                skos:prefLabel "Sustainability Report Value"@en .


###  http://www.fortiss.org/diprolea/ontosustain/rso#SOx
rso:SOx rdf:type owl:Class ;
        rdfs:subClassOf rso:OtherAirEmission ;
        rdfs:comment "Variables (measurement objects) regarding SOx."@en ;
        rdfs:isDefinedBy "https://www.globalreporting.org/publications/documents/english/gri-305-emissions-2016/" ;
        rdfs:label "SOx"@en ;
        skos:prefLabel "SOx"@en .


###  http://www.fortiss.org/diprolea/ontosustain/rso#SOxIndicator
rso:SOxIndicator rdf:type owl:Class ;
                 owl:equivalentClass [ owl:intersectionOf ( rso:OtherEmissionIndicator
                                                            [ rdf:type owl:Restriction ;
                                                              owl:onProperty rso:hasMeasurementVariable ;
                                                              owl:someValuesFrom rso:SOx
                                                            ]
                                                          ) ;
                                       rdf:type owl:Class
                                     ] ;
                 rdfs:comment "Indicator that measures SOx subtopic."@en ;
                 rdfs:label "SOx Emission Indicator"@en ;
                 skos:prefLabel "SOx Emission Indicator"@en .


###  http://www.fortiss.org/diprolea/ontosustain/rso#SocialIndicator
rso:SocialIndicator rdf:type owl:Class ;
                    owl:equivalentClass [ owl:intersectionOf ( rso:Indicator
                                                               [ rdf:type owl:Restriction ;
                                                                 owl:onProperty rso:measuresDimension ;
                                                                 owl:hasValue rso:Social
                                                               ]
                                                             ) ;
                                          rdf:type owl:Class
                                        ] ;
                    rdfs:comment "Indicators measure the social dimension of sustainability."@en ;
                    rdfs:label "Social indicator"@en ;
                    skos:prefLabel "Social indicator"@en .


###  http://www.fortiss.org/diprolea/ontosustain/rso#SoldCooling
rso:SoldCooling rdf:type owl:Class ;
                rdfs:subClassOf rso:SoldEnergy ;
                rdfs:comment "Variables (measurement objects) regarding organizational sold cooling."@en ;
                rdfs:label "Sold Cooling"@en ;
                skos:prefLabel "Sold Cooling"@en .


###  http://www.fortiss.org/diprolea/ontosustain/rso#SoldCoolingIndicator
rso:SoldCoolingIndicator rdf:type owl:Class ;
                         owl:equivalentClass [ owl:intersectionOf ( rso:SoldEnergyIndicator
                                                                    [ rdf:type owl:Restriction ;
                                                                      owl:onProperty rso:hasMeasurementVariable ;
                                                                      owl:someValuesFrom rso:SoldCooling
                                                                    ]
                                                                  ) ;
                                               rdf:type owl:Class
                                             ] ;
                         rdfs:comment "Indicator that measures sold cooling subtopic."@en ;
                         rdfs:label "Sold Cooling Indicator"@en ;
                         skos:prefLabel "Sold Cooling Indicator"@en .


###  http://www.fortiss.org/diprolea/ontosustain/rso#SoldElectricity
rso:SoldElectricity rdf:type owl:Class ;
                    rdfs:subClassOf rso:SoldEnergy ;
                    rdfs:comment "Variables (measurement objects) regarding organizational sold electricity."@en ;
                    rdfs:label "Sold Electricity"@en ;
                    skos:prefLabel "Sold Electricity"@en .


###  http://www.fortiss.org/diprolea/ontosustain/rso#SoldElectricityInidicator
rso:SoldElectricityInidicator rdf:type owl:Class ;
                              owl:equivalentClass [ owl:intersectionOf ( rso:SoldEnergyIndicator
                                                                         [ rdf:type owl:Restriction ;
                                                                           owl:onProperty rso:hasMeasurementVariable ;
                                                                           owl:someValuesFrom rso:SoldElectricity
                                                                         ]
                                                                       ) ;
                                                    rdf:type owl:Class
                                                  ] ;
                              rdfs:comment "Indicator that measures sold electricity subtopic"@en ;
                              rdfs:label "Sold Electricity Inidicator"@en ;
                              skos:prefLabel "Sold Electricity Inidicator"@en .


###  http://www.fortiss.org/diprolea/ontosustain/rso#SoldEnergy
rso:SoldEnergy rdf:type owl:Class ;
               rdfs:subClassOf rso:EnergyVariable ;
               rdfs:comment "Variables (measurement objects) regarding sold energy by the organization."@en ;
               rdfs:label "Sold Energy"@en ;
               skos:prefLabel "Sold Energy"@en .


###  http://www.fortiss.org/diprolea/ontosustain/rso#SoldEnergyIndicator
rso:SoldEnergyIndicator rdf:type owl:Class ;
                        owl:equivalentClass [ owl:intersectionOf ( rso:EnergyIndicator
                                                                   [ rdf:type owl:Restriction ;
                                                                     owl:onProperty rso:hasMeasurementVariable ;
                                                                     owl:someValuesFrom rso:SoldEnergy
                                                                   ]
                                                                 ) ;
                                              rdf:type owl:Class
                                            ] ;
                        rdfs:comment "Indicator that measures the sold energy subtopic."@en ;
                        rdfs:label "Sold Energy Indicator"@en ;
                        skos:prefLabel "Sold Energy Indicator"@en .


###  http://www.fortiss.org/diprolea/ontosustain/rso#SoldHeating
rso:SoldHeating rdf:type owl:Class ;
                rdfs:subClassOf rso:SoldEnergy ;
                rdfs:comment "Variables (measurement objects) regarding organizational sold heating."@en ;
                rdfs:label "Sold Heating"@en ;
                skos:prefLabel "Sold Heating"@en .


###  http://www.fortiss.org/diprolea/ontosustain/rso#SoldHeatingIndicator
rso:SoldHeatingIndicator rdf:type owl:Class ;
                         owl:equivalentClass [ owl:intersectionOf ( rso:SoldEnergyIndicator
                                                                    [ rdf:type owl:Restriction ;
                                                                      owl:onProperty rso:hasMeasurementVariable ;
                                                                      owl:someValuesFrom rso:SoldHeating
                                                                    ]
                                                                  ) ;
                                               rdf:type owl:Class
                                             ] ;
                         rdfs:comment "Indicator that measures sold heating subtopic."@en ;
                         rdfs:label "Sold Heating Indicator"@en ;
                         skos:prefLabel "Sold Heating Indicator"@en .


###  http://www.fortiss.org/diprolea/ontosustain/rso#SoldSteam
rso:SoldSteam rdf:type owl:Class ;
              rdfs:subClassOf rso:SoldEnergy ;
              rdfs:comment "Variables (measurement objects) regarding organizational sold steam."@en ;
              rdfs:label "Sold Steam"@en ;
              skos:prefLabel "Sold Steam"@en .


###  http://www.fortiss.org/diprolea/ontosustain/rso#SoldSteamIndicator
rso:SoldSteamIndicator rdf:type owl:Class ;
                       owl:equivalentClass [ owl:intersectionOf ( rso:SoldEnergyIndicator
                                                                  [ rdf:type owl:Restriction ;
                                                                    owl:onProperty rso:hasMeasurementVariable ;
                                                                    owl:someValuesFrom rso:SoldSteam
                                                                  ]
                                                                ) ;
                                             rdf:type owl:Class
                                           ] ;
                       rdfs:comment "Indicator that measures sold steam subtopic."@en ;
                       rdfs:label "Sold Steam Indicator"@en ;
                       skos:prefLabel "Sold Steam Indicator"@en .


###  http://www.fortiss.org/diprolea/ontosustain/rso#Standard
rso:Standard rdf:type owl:Class ;
             rdfs:comment """A sustainability reporting standard is a piece of standard that is defined by a specific standard setter. For example, the standard GRI 301: Materials 2016 is part of the GRI Sustainability Reporting Standards (GRI Standards).
This class is defined as the super class for subclasses."""@en ;
             rdfs:label "Sustainability Standard"@en ;
             skos:prefLabel "Sustainability Standard"@en .


###  http://www.fortiss.org/diprolea/ontosustain/rso#StandardSet
rso:StandardSet rdf:type owl:Class ;
                rdfs:comment "Models a series of sustainability reporting standards."@en ;
                rdfs:label "Standard Set"@en ;
                skos:prefLabel "Standard Set"@en .


###  http://www.fortiss.org/diprolea/ontosustain/rso#Topic
rso:Topic rdf:type owl:Class ;
          rdfs:comment "delineates sustainability issues."@en ;
          rdfs:label "Sustainability Topic"@en ;
          skos:prefLabel "Sustainability Topic"@en .


###  http://www.fortiss.org/diprolea/ontosustain/rso#VOC
rso:VOC rdf:type owl:Class ;
        rdfs:subClassOf rso:OtherAirEmission ;
        rdfs:comment "Variables (measurement objects) regarding VOC."@en ;
        rdfs:isDefinedBy "https://www.globalreporting.org/publications/documents/english/gri-305-emissions-2016/" ;
        rdfs:label "Volatile organic compounds (VOC)"@en ;
        skos:prefLabel "Volatile organic compounds (VOC)"@en .


###  http://www.fortiss.org/diprolea/ontosustain/rso#VOCIndicator
rso:VOCIndicator rdf:type owl:Class ;
                 owl:equivalentClass [ owl:intersectionOf ( rso:OtherEmissionIndicator
                                                            [ rdf:type owl:Restriction ;
                                                              owl:onProperty rso:hasMeasurementVariable ;
                                                              owl:someValuesFrom rso:VOC
                                                            ]
                                                          ) ;
                                       rdf:type owl:Class
                                     ] ;
                 rdfs:comment "Indicator that measures Volatile organic compounds (VOC) subtopic"@en ;
                 rdfs:label "Volatile organic compounds (VOC) indicator"@en ;
                 skos:prefLabel "Volatile organic compounds (VOC) Indicator"@en .


###  http://www.fortiss.org/diprolea/ontosustain/rso#Value
rso:Value rdf:type owl:Class ;
          rdfs:comment "This class acts as a collective framework for organizing quantitative data within sustainability reports. It encompasses two subclasses:(1) ReportValue, which structures individual data entries including numerical values and units linked to specific indicators, and (2) BreakdownValue, which allows for detailed disaggregation of data according to defined criteria, enhancing data analysis and reporting precision."@en ;
          rdfs:label "Value"@en ;
          skos:prefLabel "Value"@en .


###  http://www.fortiss.org/diprolea/ontosustain/rso#Variable
rso:Variable rdf:type owl:Class ;
             rdfs:comment "A variable encompasses a hierarchy of subtopics within specific sustainability areas. It represents a measurable value of a phenomenon, like 'total energy consumption'."@en ;
             rdfs:label "Sustainability Variable"@en ;
             skos:prefLabel "Sustainability Variable"@en .


###  http://www.fortiss.org/diprolea/ontosustain/rso#Waste
rso:Waste rdf:type owl:Class ;
          rdfs:subClassOf rso:Variable ;
          rdfs:comment "A variable that quantifies waste metrics."@en ;
          rdfs:label "Waste"@en ;
          skos:prefLabel "Waste"@en .


###  http://www.fortiss.org/diprolea/ontosustain/rso#WasteDFDIndicator
rso:WasteDFDIndicator rdf:type owl:Class ;
                      owl:equivalentClass [ owl:intersectionOf ( rso:WasteIndicator
                                                                 [ rdf:type owl:Restriction ;
                                                                   owl:onProperty rso:hasMeasurementVariable ;
                                                                   owl:someValuesFrom rso:WasteDivertedFromDisposal
                                                                 ]
                                                               ) ;
                                            rdf:type owl:Class
                                          ] ;
                      rdfs:comment "Indicator that measures the waste diverted from disposal subtopic."@en ;
                      rdfs:label "Diverted From Disposal Waste Inidicator"@en ;
                      skos:prefLabel "Diverted From Disposal Waste Inidicator"@en .


###  http://www.fortiss.org/diprolea/ontosustain/rso#WasteDTDIndicator
rso:WasteDTDIndicator rdf:type owl:Class ;
                      owl:equivalentClass [ owl:intersectionOf ( rso:WasteIndicator
                                                                 [ rdf:type owl:Restriction ;
                                                                   owl:onProperty rso:hasMeasurementVariable ;
                                                                   owl:someValuesFrom rso:WasteDirectedToDisposal
                                                                 ]
                                                               ) ;
                                            rdf:type owl:Class
                                          ] ;
                      rdfs:comment "Indicator that measures the waste directed to disposal subtopic."@en ;
                      rdfs:label "Directed To Disposal Waste Indicator"@en ;
                      skos:prefLabel "Directed To Disposal Waste Indicator"@en .


###  http://www.fortiss.org/diprolea/ontosustain/rso#WasteDirectedToDisposal
rso:WasteDirectedToDisposal rdf:type owl:Class ;
                            rdfs:subClassOf rso:Waste ;
                            rdfs:comment "Variables (measurement objects) regarding waste directed to disposal."@en ;
                            rdfs:label "Waste Directed To Disposal"@en ;
                            skos:prefLabel "Waste Directed To Disposal"@en .


###  http://www.fortiss.org/diprolea/ontosustain/rso#WasteDivertedFromDisposal
rso:WasteDivertedFromDisposal rdf:type owl:Class ;
                              rdfs:subClassOf rso:Waste ;
                              rdfs:comment "Variables (measurement objects) regarding waste diverted from disposal."@en ;
                              rdfs:label "Waste Diverted From Disposal"@en ;
                              skos:prefLabel "Waste Diverted From Disposal"@en .


###  http://www.fortiss.org/diprolea/ontosustain/rso#WasteIndicator
rso:WasteIndicator rdf:type owl:Class ;
                   owl:equivalentClass [ owl:intersectionOf ( rso:Indicator
                                                              [ rdf:type owl:Restriction ;
                                                                owl:onProperty rso:hasMeasurementVariable ;
                                                                owl:someValuesFrom rso:Waste
                                                              ]
                                                            ) ;
                                         rdf:type owl:Class
                                       ] ;
                   rdfs:comment "Indicators measure the waste topic."@en ;
                   rdfs:label "Waste Indicator"@en ;
                   skos:prefLabel "Waste Indicator"@en .


###  http://www.fortiss.org/diprolea/ontosustain/rso#WeightedIndicator
rso:WeightedIndicator rdf:type owl:Class ;
                      rdfs:subClassOf rso:Indicator ;
                      rdfs:comment "Weighted indicator considers additional factors through weighting."@en ;
                      rdfs:label "Weighted Indicator"@en ;
                      skos:prefLabel "Weighted Indicator"@en .


###  http://www.w3.org/ns/org#Organization
<http://www.w3.org/ns/org#Organization> rdf:type owl:Class .


#################################################################
#    Individuals
#################################################################

###  http://www.fortiss.org/diprolea/ontosustain/rso#Environment
rso:Environment rdf:type owl:NamedIndividual ,
                         rso:ESGDimension ;
                rdfs:comment "Emissions such as greenhouse gases and air, water and ground pollution emissions falls under the Environmental dimension of sustainability."@en ;
                rdfs:label "Environmental (E)"@en ;
                skos:prefLabel "Environmental (E)"@en .


###  http://www.fortiss.org/diprolea/ontosustain/rso#Governance
rso:Governance rdf:type owl:NamedIndividual ,
                        rso:ESGDimension ;
               rdfs:comment "The main issues reported under the Governance Pillar are shareholders rights, board diversity, how executives are compensated and how their compensation is aligned with the company’s sustainability performance. It also includes matters of corporate behaviour such as anti-competitive practices and corruption."@en ;
               rdfs:label "Coporate Governance (G)"@en ;
               skos:prefLabel "Coporate Governance (G)" .


###  http://www.fortiss.org/diprolea/ontosustain/rso#Social
rso:Social rdf:type owl:NamedIndividual ,
                    rso:ESGDimension ;
           rdfs:comment "Under the Social dimension, companies report on how they manage their employee development and labour practices."@en ;
           rdfs:label "Social (S)"@en ;
           skos:prefLabel "Social (S)"@en .


###  http://www.fortiss.org/diprolea/ontosustain/rso#enumerated
rso:enumerated rdf:type owl:NamedIndividual ,
                        rso:Applicability ;
               rdfs:comment """An enumerated requirement is described as \"the organization shall report on the information of A or B of a phenomenon\".
For example, \"the reporting organization shall report the following information: total weight or volume of materials that are used to produce .....\", refering to GRI 301-1."""@en ;
               rdfs:label "enumerated"@en ;
               skos:prefLabel "enumerated"@en .


###  http://www.fortiss.org/diprolea/ontosustain/rso#mandatory
rso:mandatory rdf:type owl:NamedIndividual ,
                       rso:Applicability ;
              rdfs:comment "A mandatory requirement for an indicator is indicated by the word \"shall\" in the requirement description."@en ;
              rdfs:label "mandatory"@en ;
              skos:prefLabel "mandatory"@en .


###  http://www.fortiss.org/diprolea/ontosustain/rso#optional
rso:optional rdf:type owl:NamedIndividual ,
                      rso:Applicability ;
             rdfs:comment "An optional requirement for an indicator is indicated by the expression \"if applicable\" in the requirement description."@en ;
             rdfs:label "optional"@en ;
             skos:prefLabel "optional"@en .


#################################################################
#    General axioms
#################################################################

[ rdf:type owl:AllDisjointClasses ;
  owl:members ( rso:CoreEnvironmentTopic
                rso:CoreGovernanceTopic
                rso:CoreSocialTopic
              )
] .


[ rdf:type owl:AllDisjointClasses ;
  owl:members ( rso:ESRSEnvironmentTopic
                rso:ESRSGovernanceTopic
                rso:ESRSSocialTopic
              )
] .


[ rdf:type owl:AllDisjointClasses ;
  owl:members ( rso:GRIEnvironmentTopic
                rso:GRIGovernanceTopic
                rso:GRISocialTopic
              )
] .


###  Generated by the OWL API (version 4.5.26.2023-07-17T20:34:13Z) https://github.com/owlcs/owlapi
